
\documentclass{article}

\usepackage{amsmath}
\usepackage{ebproof}
\usepackage{fullpage}
\usepackage[utf8]{inputenc}
\usepackage{newunicodechar}
\usepackage{stix}

\newunicodechar{Γ}{\Gamma}
\newunicodechar{Δ}{\Delta}

\newunicodechar{⊢}{\vdash}

\newunicodechar{∀}{\forall}
\newunicodechar{∃}{\exists}

\newunicodechar{⊕}{\oplus}
\newunicodechar{¬}{\neg}

\setlength{\parindent}{0em}

\author{James Martin, Ian D.L.N. Mclean}
\title{First Order Additive Sequent Calculus}

\begin{document}

\maketitle

\begin{abstract}
Strictly visible additive order calculus with first order quantification.
\end{abstract}

\section{Structural Rules}

\begin{center}
	\[
	\begin{prooftree}
	\infer0[Id]{A ⊢ A}
	\end{prooftree}
	\]
	
	\[
	\begin{prooftree}
	\hypo{Γ ⊢ A}
	\hypo{A ⊢ Δ}
	\infer2[cut]{Γ ⊢ Δ}
	\end{prooftree}
	\]
\end{center}

\section{Quantifiers}
	\begin{center}
		Standard Eigenvariable Condition Quantifiers
		\[
		\begin{prooftree}
		\hypo{P[t/x] ⊢ Δ}
		\infer1{∀x.P(x) ⊢ Δ}
		\end{prooftree}
		\quad
		\begin{prooftree}
		\hypo{Γ ⊢ P[y/x]}
		\infer1{Γ ⊢ ∀x.P(x)}
		\end{prooftree}
		\]
		in $∀R$ the variable y must not occur free anywhere in the lower sequent.
		\[
		\begin{prooftree}
		\hypo{P[y/x] ⊢ Δ}
		\infer1{∃x.P(x) ⊢ Δ}
		\end{prooftree}
		\quad
		\begin{prooftree}
		\hypo{Γ ⊢ P[t/x]}
		\infer1{Γ ⊢ ∃x.P(x)}
		\end{prooftree}
		\]
		in $∃L$ the variable y must not occur free anywhere in the lower sequent.
		\[
		\begin{prooftree}
		\hypo{P(y)⊢}
		\infer1{¬∀x.¬P(x) ⊢ }
		\end{prooftree}
		\quad
		\begin{prooftree}
		\hypo{⊢P(t)}
		\infer1{⊢ ¬∀x.¬P(x)}
		\end{prooftree}
		\quad
		\begin{prooftree}
		\hypo{P(t)⊢}
		\infer1{¬∃x.¬P(x) ⊢ }
		\end{prooftree}
		\quad
		\begin{prooftree}
		\hypo{⊢P(y)}
		\infer1{⊢ ¬∃x.¬P(x)}
		\end{prooftree}
		\]
		
		
		Henkin constant quantifiers
		\[
		\begin{prooftree}
		\hypo{P[t/x] ⊢ Δ}
		\infer1{∀x.P ⊢ Δ}
		\end{prooftree}
		\quad
		\begin{prooftree}
		\hypo{Γ ⊢ P [c_{∀x.P}/x]}
		\infer1{Γ ⊢ ∀x.P}
		\end{prooftree}
		\]
		
		\[
		\begin{prooftree}
		\hypo{P[c_{∃x.P}/x] ⊢ Δ}
		\infer1{∃xP ⊢ Δ}
		\end{prooftree}
		\quad
		\begin{prooftree}
		\hypo{Γ ⊢ P[t/x]}
		\infer1{Γ ⊢ ∃xP}
		\end{prooftree}
		\]
		
		\[
		\begin{prooftree}
		\hypo{P(t/x) ⊢ Δ}
		\infer1{∀xP(x) ⊢ Δ}
		\end{prooftree}
		\quad
		\begin{prooftree}
		\hypo{Γ ⊢ P (c_{∀x.P}/x)}
		\infer1{Γ ⊢ ∀xP(x)}
		\end{prooftree}
		\]
		
		\[
		\begin{prooftree}
		\hypo{P(c_{∃x.P}/x) ⊢ Δ}
		\infer1{∃xP(x) ⊢ Δ}
		\end{prooftree}
		\quad
		\begin{prooftree}
		\hypo{Γ ⊢ P(t/x)}
		\infer1{Γ ⊢ ∃xP(x)}
		\end{prooftree}
		\]
	\end{center}

\section{Operational Rules}
	\begin{center}
				\subsection{Negation}
				\begin{center}
					\[
					\begin{prooftree}
					\hypo{ ⊢ A}
					\infer1{¬ A ⊢}
					\end{prooftree}
					\quad
					\begin{prooftree}
					\hypo{A ⊢ }
					\infer1{⊢ ¬ A}
					\end{prooftree}
					\]
				\end{center}
				
				
				\subsection{Negative Junctions}
				\begin{center}
					\[
					\begin{prooftree}
					\hypo{⊢ A}
					\hypo{⊢ B}
					\infer2{¬A ⊕ ¬B ⊢ }
					\end{prooftree}
					\quad
					\begin{prooftree}
					\hypo{A ⊢ }
					\infer1{ ⊢ ¬A ⊕ ¬B}
					\end{prooftree}
					\quad
					\begin{prooftree}
					\hypo{B ⊢ }
					\infer1{ ⊢ ¬A ⊕ ¬B}
					\end{prooftree}
					\]
					
					\[
					\begin{prooftree}
					\hypo{⊢ B}
					\hypo{ ⊢ A}
					\infer2{¬B ⊕ ¬A ⊢ }
					\end{prooftree}
					\quad
					\begin{prooftree}
					\hypo{A ⊢ }
					\infer1{ ⊢ ¬B ⊕ ¬A}
					\end{prooftree}
					\quad
					\begin{prooftree}
					\hypo{B ⊢ }
					\infer1{ ⊢ ¬B ⊕ ¬A}
					\end{prooftree}
					\]
					
					\[
					\begin{prooftree}
					\hypo{ ⊢ A}
					\infer1{¬A \& ¬B ⊢ }
					\end{prooftree}
					\quad
					\begin{prooftree}
					\hypo{ ⊢ B}
					\infer1{¬A \& ¬B ⊢ }
					\end{prooftree}
					\quad
					\begin{prooftree}
					\hypo{A ⊢ }
					\hypo{B ⊢ }
					\infer2{⊢ ¬A \& ¬B}
					\end{prooftree}
					\]
					
					\[
					\begin{prooftree}
					\hypo{ ⊢ A}
					\infer1{¬B \& ¬A ⊢ }
					\end{prooftree}
					\quad
					\begin{prooftree}
					\hypo{ ⊢ B}
					\infer1{¬B \& ¬A ⊢ }
					\end{prooftree}
					\quad
					\begin{prooftree}
					\hypo{B ⊢ }
					\hypo{A ⊢ }
					\infer2{ ⊢ ¬ B \& ¬ A}
					\end{prooftree}
					\]
				\end{center}

				\subsection{Conditionals}
				\begin{center}
					\[
					\begin{prooftree}
					\hypo{⊢ B}
					\hypo{A ⊢ }
					\infer2{¬B ⊕ A ⊢}
					\end{prooftree}
					\quad
					\begin{prooftree}
					\hypo{A ⊢ }
					\hypo{⊢ B}
					\infer2{A ⊕ ¬B ⊢}
					\end{prooftree}
					\quad
					\begin{prooftree}
					\hypo{Γ ⊢ A}
					\infer1{Γ ⊢ A ⊕ ¬B}
					\end{prooftree}
					\quad
					\begin{prooftree}
					\hypo{B ⊢ }
					\infer1{⊢ A ⊕ ¬B}
					\end{prooftree}
					\]
					
					\[
					\begin{prooftree}
					\hypo{ ⊢ A}
					\hypo{B ⊢ }
					\infer2{¬A ⊕ B ⊢ }
					\end{prooftree}
					\quad
					\begin{prooftree}
					\hypo{B ⊢ }
					\hypo{ ⊢ A}
					\infer2{B ⊕ ¬A ⊢ }
					\end{prooftree}
					\quad
					\begin{prooftree}
					\hypo{A ⊢ }
					\infer1{ ⊢ B ⊕ ¬A}
					\end{prooftree}
					\quad
					\begin{prooftree}
					\hypo{Γ ⊢ B}
					\infer1{Γ ⊢ B ⊕ ¬A}
					\end{prooftree}
					\]
					
					\[
					\begin{prooftree}
					\hypo{A ⊢ Δ}
					\infer1{A \& ¬B ⊢ Δ}
					\end{prooftree}
					\quad
					\begin{prooftree}
					\hypo{ ⊢ B}
					\infer1{A \& ¬B ⊢ }
					\end{prooftree}
					\quad
					\begin{prooftree}
					\hypo{⊢ A}
					\hypo{B ⊢ }
					\infer2{⊢ A \& ¬B}
					\end{prooftree}
					\quad
					\begin{prooftree}
					\hypo{B ⊢ }
					\hypo{⊢ A}
					\infer2{⊢ ¬B \& A}
					\end{prooftree}
					\]
					
					\[
					\begin{prooftree}
					\hypo{ ⊢ A}
					\infer1{B \& ¬A ⊢ }
					\end{prooftree}
					\quad
					\begin{prooftree}
					\hypo{B ⊢ Δ}
					\infer1{B \& ¬A ⊢ Δ}
					\end{prooftree}
					\quad
					\begin{prooftree}
					\hypo{ ⊢ B}
					\hypo{A ⊢ }
					\infer2{ ⊢ B \& ¬ A}
					\end{prooftree}
					\quad
					\begin{prooftree}
					\hypo{A ⊢ }
					\hypo{ ⊢ B}
					\infer2{ ⊢ ¬A \& B}
					\end{prooftree}
					\]
				\end{center}
				
				\subsection{Junctions}
				\begin{center}
					\[
					\begin{prooftree}
					\hypo{A ⊢ Δ}
					\hypo{B ⊢ Δ}
					\infer2{A ⊕ B ⊢ Δ}
					\end{prooftree}
					\quad
					\begin{prooftree}
					\hypo{Γ ⊢ A}
					\infer1{Γ ⊢ A ⊕ B}
					\end{prooftree}
					\quad
					\begin{prooftree}
					\hypo{Γ ⊢ B}
					\infer1{Γ ⊢ A ⊕ B}
					\end{prooftree}
					\]
					
					\[
					\begin{prooftree}
					\hypo{B ⊢ Δ}
					\hypo{A ⊢ Δ}
					\infer2{B ⊕ A ⊢ Δ}
					\end{prooftree}
					\quad
					\begin{prooftree}
					\hypo{Γ ⊢ A}
					\infer1{Γ ⊢ B ⊕ A}
					\end{prooftree}
					\quad
					\begin{prooftree}
					\hypo{Γ ⊢ B}
					\infer1{Γ ⊢ B ⊕ A}
					\end{prooftree}
					\]
					
					\[
					\begin{prooftree}
					\hypo{A ⊢ Δ}
					\infer1{A \& B ⊢ Δ}
					\end{prooftree}
					\quad
					\begin{prooftree}
					\hypo{B ⊢ Δ}
					\infer1{A \& B ⊢ Δ}
					\end{prooftree}
					\quad
					\begin{prooftree}
					\hypo{Γ ⊢ A}
					\hypo{Γ ⊢ B}
					\infer2{Γ ⊢ A \& B}
					\end{prooftree}
					\]
					
					\[
					\begin{prooftree}
					\hypo{A ⊢ Δ}
					\infer1{B \& A ⊢ Δ}
					\end{prooftree}
					\quad
					\begin{prooftree}
					\hypo{B ⊢ Δ}
					\infer1{B \& A ⊢ Δ}
					\end{prooftree}
					\quad
					\begin{prooftree}
					\hypo{Γ ⊢ B}
					\hypo{Γ ⊢ A}
					\infer2{Γ ⊢ B \& A}
					\end{prooftree}
					\]
				\end{center}
			
				\subsection{Biconditionals}
				\begin{center}
					\[
					\begin{prooftree}
					\hypo{⊢ A}
					\hypo{B ⊢ }
					\infer2{(¬A ⊕ B) \& (¬B ⊕ A) ⊢ }
					\end{prooftree}
					\quad
					\begin{prooftree}
					\hypo{⊢ B}
					\hypo{A ⊢ }
					\infer2{(¬A ⊕ B) \& (¬B ⊕ A) ⊢ }
					\end{prooftree}
					\quad
					\begin{prooftree}
					\hypo{A ⊢ }
					\hypo{B ⊢ }
					\infer2{ ⊢ (¬A ⊕ B) \& (¬B ⊕ A)}
					\end{prooftree}
					\quad
					\begin{prooftree}
					\hypo{Γ ⊢ B}
					\hypo{Γ ⊢ A}
					\infer2{Γ ⊢ (¬A ⊕ B) \& (¬B ⊕ A)}
					\end{prooftree}
					\]
					
					\[
					\begin{prooftree}
					\hypo{A ⊢ }
					\hypo{⊢A}
					\infer2{(A \& B) ⊕  (¬A \& ¬B) ⊢ }
					\end{prooftree}
					\quad
					\begin{prooftree}
					\hypo{A ⊢ }
					\hypo{⊢B}
					\infer2{(A \& B) ⊕  (¬A \& ¬B) ⊢ }
					\end{prooftree}
					\quad
					\begin{prooftree}
					\hypo{B ⊢ }
					\hypo{⊢A}
					\infer2{(A \& B) ⊕  (¬A \& ¬B) ⊢ }
					\end{prooftree}
					\quad
					\begin{prooftree}
					\hypo{B ⊢ }
					\hypo{⊢B}
					\infer2{(A \& B) ⊕  (¬A \& ¬B) ⊢ }
					\end{prooftree}
					\]
					
					\[
					\quad
					\begin{prooftree}
					\hypo{Γ ⊢ A}
					\hypo{Γ ⊢ B}
					\infer2{Γ ⊢ (A \& B) ⊕  (¬A \& ¬B)}
					\end{prooftree}
					\quad
					\begin{prooftree}
					\hypo{B ⊢ }
					\hypo{A ⊢ }
					\infer2{ ⊢ (A \& B) ⊕  (¬A \& ¬B)}
					\end{prooftree}
					\]
					
					TODO: XOR-like
				\end{center}
\end{center}

\part{Theorems}
	\begin{center}
		\[
		\begin{prooftree}
		\infer0{P(c_{∀x∃y.P(x,y)},c_{∃y∀x.P(x,y)}) ⊢ P(c_{∀x∃y.P(x,y)},c_{∃y∀x.P(x,y)})}
		\infer1{P(c_{∀x∃y.P(x,y)},c_{∃y∀x.P(x,y)}) ⊢ ∃y.P(c_{∀x∃y.P(x,y)},y)}
		\infer1{∀x.P(x,c_{∃y∀x.P(x,y)}) ⊢ ∃y.P(c_{∀x∃y.P(x,y)},y)}
		\infer1{∀x.P(x,c_{∃y∀x.P(x,y)}) ⊢ ∀x∃y.P(x,y)}
		\infer1{∃y∀x.P(x,y) ⊢ ∀x∃y.P(x,y)}
		\end{prooftree}
		\]
	\end{center}

\end{document}
