
\documentclass{article}

\usepackage{amsmath}
\usepackage{ebproof}
\usepackage{fullpage}
\usepackage[utf8]{inputenc}
\usepackage{newunicodechar}
\usepackage{stix}

\newunicodechar{Γ}{\Gamma}
\newunicodechar{Δ}{\Delta}

\newunicodechar{Θ}{\Theta}
\newunicodechar{Λ}{\Lambda}

\newunicodechar{Ξ}{\Xi}
\newunicodechar{Π}{\Pi}

\newunicodechar{Φ}{\Phi}
\newunicodechar{Ψ}{\Psi}

\newunicodechar{Ω}{\Omega}

\newunicodechar{⊢}{\vdash}

\newunicodechar{⊕}{\oplus}
\newunicodechar{¬}{\neg}

\newunicodechar{⊗}{\otimes}
\newunicodechar{→}{\rightarrow}
\newunicodechar{←}{\leftarrow}

\newunicodechar{⅋}{\upand}
\newunicodechar{↛}{\nrightarrow}
\newunicodechar{↚}{\nleftarrow}

\newunicodechar{⊥}{\bot}
\newunicodechar{⊤}{\top}

\setlength{\parindent}{0em}

\author{James Martin, Ian D.L.N. Mclean}
\title{Ordinary Multiplicative Calculus}

\begin{document}

\maketitle

\begin{abstract}
A sequent calculus of ordinary multiplicatives.
\end{abstract}

\section{Structural Rules}

\begin{center}
	\[
	\begin{prooftree}
	\infer0[Id]{A ⊢ A}
	\end{prooftree}
	\]
	
	\[
	\begin{prooftree}
	\hypo{Γ_{L}, A ⊢}
	\hypo{⊢ Δ_{L}, A}
	\infer2[Cut]{Γ_{L} ⊢ Δ_{L}}
	\end{prooftree}
	\]
	
	\[
	\begin{prooftree}
	\hypo{A, Γ_{R} ⊢}
	\hypo{⊢ A, Δ_{R}}
	\infer2[Cut]{Γ_{R} ⊢ Δ_{R}}
	\end{prooftree}
	\]
	\[
	\begin{prooftree}
	\hypo{Γ ⊢ A}
	\hypo{A ⊢ Δ}
	\infer2[Cut]{Γ ⊢ Δ}
	\end{prooftree}
	\]
	
	\[
	\begin{prooftree}
	\hypo{Γ_{L}, A, Γ_{R} ⊢}
	\hypo{⊢ Δ_{L}, A, Δ_{R}}
	\infer2[Cut]{Γ_{L}, Γ_{R} ⊢ Δ_{L}, Δ_{R}}
	\end{prooftree}
	\]
	
	\[
	\begin{prooftree}
	\hypo{Γ_{L}, A, Γ_{R} ⊢ Δ_{M}}
	\hypo{Γ_{M} ⊢ Δ_{L}, A, Δ_{R}}
	\infer2[Cut]{Γ_{L}, Γ_{M}, Γ_{R} ⊢ Δ_{L}, Δ_{M}, Δ_{R}}
	\end{prooftree}
	\]
\end{center}

\newpage
\section{Operational Rules}
\begin{center}
	\subsection{Negations}
	\begin{center}
		\[
		\begin{prooftree}
		\hypo{Γ_{L}, Γ_{R} ⊢ Δ_{L}, A, Δ_{R}}
		\infer1{Γ_{L}, ¬_{M} A, Γ_{R} ⊢ Δ_{L}, Δ_{R}}
		\end{prooftree}
		\quad
		\begin{prooftree}
		\hypo{ Γ_{L}, A, Γ_{R} ⊢ Δ_{L}, Δ_{R}}
		\infer1{ Γ_{L}, Γ_{R} ⊢ Δ_{L}, ¬_{M} A, Δ_{R}}
		\end{prooftree}
		\]
		
		\[
		\begin{prooftree}
		\hypo{Γ_{L}, Γ_{R} ⊢ A, Δ}
		\infer1{Γ_{L}, ¬_{L} A, Γ_{R} ⊢ Δ}
		\end{prooftree}
		\quad
		\begin{prooftree}
		\hypo{A, Γ ⊢ Δ_{L}, Δ_{R}}
		\infer1{ Γ ⊢ Δ_{L}, ¬_{L} A, Δ_{R}}
		\end{prooftree}
		\]
		
		\[
		\begin{prooftree}
		\hypo{Γ_{L}, Γ_{R} ⊢ Δ, A}
		\infer1{Γ_{L}, ¬_{R} A, Γ_{R} ⊢ Δ}
		\end{prooftree}
		\quad
		\begin{prooftree}
		\hypo{ Γ, A ⊢ Δ_{L}, Δ_{R}}
		\infer1{ Γ ⊢ Δ_{L}, ¬_{R} A, Δ_{R}}
		\end{prooftree}
		\]
		
		\[
		\begin{prooftree}
		\hypo{Γ ⊢ A, Δ}
		\infer1{¬_{L} A, Γ ⊢ Δ}
		\end{prooftree}
		\quad
		\begin{prooftree}
		\hypo{ A, Γ ⊢ Δ}
		\infer1{ Γ ⊢ ¬_{L} A, Δ}
		\end{prooftree}
		\quad
		\begin{prooftree}
		\hypo{Γ ⊢ Δ, A}
		\infer1{Γ, ¬_{R} A ⊢ Δ}
		\end{prooftree}
		\quad
		\begin{prooftree}
		\hypo{ Γ, A ⊢ Δ}
		\infer1{ Γ ⊢ Δ, ¬_{R} A}
		\end{prooftree}
		\]
		
		\[
		\begin{prooftree}
		\hypo{Γ ⊢ Δ, A}
		\infer1{¬^{*}_{L} A, Γ ⊢ Δ}
		\end{prooftree}
		\quad
		\begin{prooftree}
		\hypo{Γ, A ⊢ Δ}
		\infer1{ Γ ⊢ ¬^{*}_{L} A, Δ}
		\end{prooftree}
		\quad
		\begin{prooftree}
		\hypo{Γ ⊢ A, Δ}
		\infer1{Γ, ¬^{*}_{R} A ⊢ Δ}
		\end{prooftree}
		\quad
		\begin{prooftree}
		\hypo{ A, Γ ⊢ Δ}
		\infer1{ Γ ⊢ Δ, ¬^{*}_{R} A}
		\end{prooftree}
		\]
	\end{center}

	\subsection{Junctions}
	\begin{center}
		\[
		\begin{prooftree}
		\hypo{Γ_{L}, A, B, Γ_{R} ⊢ Δ}
		\infer1{Γ_{L}, A ⊗ B, Γ_{R} ⊢ Δ}
		\end{prooftree}
		\quad
		\begin{prooftree}
		\hypo{Γ_{L} ⊢ Δ_{L}, A}
		\hypo{Γ_{R} ⊢ B, Δ_{R}}
		\infer2{Γ_{L}, Γ_{R} ⊢ Δ_{L}, A ⊗ B, Δ_{R}}
		\end{prooftree}
		\]
		
		\[
		\begin{prooftree}
		\hypo{Γ_{L}, B, A, Γ_{R} ⊢ Δ}
		\infer1{Γ_{L}, B ⊗ A, Γ_{R} ⊢ Δ}
		\end{prooftree}
		\quad
		\begin{prooftree}
		\hypo{Γ_{L} ⊢ Δ_{L}, B}
		\hypo{Γ_{R} ⊢ A, Δ_{R}}
		\infer2{Γ_{L}, Γ_{R} ⊢ Δ_{L}, B ⊗ A, Δ_{R}}
		\end{prooftree}
		\]
		
		\[
		\begin{prooftree}
		\hypo{Γ_{L}, B ⊢ Δ_{L}}
		\hypo{A, Γ_{R} ⊢ Δ_{R}}
		\infer2{Γ_{L}, B ⅋ A, Γ_{R} ⊢ Δ_{L}, Δ_{R}}
		\end{prooftree}
		\quad
		\begin{prooftree}
		\hypo{Γ ⊢ Δ_{L}, B, A, Δ_{R}}
		\infer1{Γ ⊢ Δ_{L}, B ⅋ A, Δ_{R}}
		\end{prooftree}
		\]
		
		\[
		\begin{prooftree}
		\hypo{Γ_{L}, A ⊢ Δ_{L}}
		\hypo{B, Γ_{R} ⊢ Δ_{R}}
		\infer2{Γ_{L}, A ⅋ B, Γ_{R} ⊢ Δ_{L}, Δ_{R}}
		\end{prooftree}
		\quad
		\begin{prooftree}
		\hypo{Γ ⊢ Δ_{L}, A, B, Δ_{R}}
		\infer1{Γ ⊢ Δ_{L}, A ⅋ B, Δ_{R}}
		\end{prooftree}
		\]
	\end{center}
	\subsection{Conditionals}
		\begin{center}
			There are at least 4 kinds of implications possibly 5 if middle negation can be used. 
		\end{center}
		\subsection{Biconditionals}
			\begin{center}
				\[
				\begin{prooftree}
				\hypo{Γ_{L}, ¬A ⅋ B, ¬B ⅋ A, Γ_{R} ⊢ Δ_{L},Δ_{M},Δ_{R}}
				\infer1{Γ_{L}, (¬A ⅋ B)⊗(¬B ⅋ A), Γ_{R} ⊢ Δ_{L},Δ_{M},Δ_{R}}
				\end{prooftree}
				\quad
				\begin{prooftree}
				\hypo{Γ_{L}, ¬A ⊢ Δ_{L}}
				\hypo{B, ¬B ⊢ Δ_{M}}
				\hypo{A, Γ_{R} ⊢ Δ_{R}}
				\infer3{Γ_{L}, (¬A ⅋ B)⊗(¬B ⅋ A), Γ_{R} ⊢ Δ_{L},Δ_{M},Δ_{R}}
				\end{prooftree}
				\]
				
				\[
				\begin{prooftree}
				\hypo{Γ_{L} ⊢ Δ_{L}, ¬A , B}
				\hypo{Γ_{R} ⊢ ¬B , A, Δ_{R}}
				\infer2{Γ_{L}, Γ_{R} ⊢ Δ_{L}, (¬A ⅋ B)⊗(¬B ⅋ A), Δ_{R}}
				\end{prooftree}
				\]
				
				\[
				\begin{prooftree}
				\hypo{A, Γ_{L} ⊢ Δ_{L}, B}
				\hypo{B, Γ_{R} ⊢ A, Δ_{R}}
				\infer2{Γ_{L}, Γ_{R} ⊢ Δ_{L}, (¬_{L}A ⅋ B)⊗(¬_{L}B ⅋ A), Δ_{R}}
				\end{prooftree}
				\]
				
				\[
				\begin{prooftree}
				\hypo{Γ_{L}, A ⊢ Δ_{L}, B}
				\hypo{Γ_{R}, B ⊢ A, Δ_{R}}
				\infer2{Γ_{L}, Γ_{R} ⊢ Δ_{L}, (¬_{R}A ⅋ B)⊗(¬_{R}B ⅋ A), Δ_{R}}
				\end{prooftree}
				\]
				
				\[
				\begin{prooftree}
				\hypo{Γ_{L}, A , B ⊢ Δ_{L}}
				\hypo{¬A , ¬B, Γ_{R} ⊢ Δ_{R}}
				\infer2{Γ_{L}, (A ⊗ B)⅋(¬A ⊗ ¬B), Γ_{R} ⊢ Δ_{L},Δ_{R}}
				\end{prooftree}
				\]
			\end{center}
\end{center}

\part{Theorems}
	\begin{center}
		
	\end{center}

\end{document}
