
\documentclass{article}

\usepackage{amsmath}
\usepackage{ebproof}
\usepackage{fullpage}
\usepackage[utf8]{inputenc}
\usepackage{newunicodechar}
\usepackage{stix}

\newunicodechar{Γ}{\Gamma}
\newunicodechar{Δ}{\Delta}
\newunicodechar{Π}{\Pi}
\newunicodechar{Λ}{\Lambda}
\newunicodechar{Θ}{\Theta}

\newunicodechar{⊢}{\vdash}

\newunicodechar{℘}{\wp}
\newunicodechar{⊗}{\otimes}
\newunicodechar{⊕}{\oplus}
\newunicodechar{¬}{\neg}

\newunicodechar{→}{\rightarrow}

\newunicodechar{⊥}{\bot}
\newunicodechar{⊤}{\top}

\setlength{\parindent}{0em}

\author{James Martin, Ian D.L.N. Mclean}
\title{Ordinary Additive Sequent Calculus with Partial Visibility}

\begin{document}

\maketitle

\begin{abstract}
Negation has partial visibility; the junctions obey strict visibility but the conditionals obey partial visibility.
\end{abstract}
	\begin{center}
		\section{Structural Rules}
			\begin{center}
				\[
				\begin{prooftree}
				\infer0[Id]{A ⊢ A}
				\end{prooftree}
				\]
				
				\[
				\begin{prooftree}
				\hypo{Γ ⊢ A}
				\hypo{A ⊢ Δ}
				\infer2[cut]{Γ ⊢ Δ}
				\end{prooftree}
				\]
			\end{center}
		
		\section{Operational Rules}
			\begin{center}
				Negations
				\[
				\begin{prooftree}
				\hypo{ ⊢ Δ, A}
				\infer1{¬_{R} A ⊢ Δ}
				\end{prooftree}
				\quad
				\begin{prooftree}
				\hypo{Γ, A ⊢ }
				\infer1{Γ ⊢ ¬_{R} A}
				\end{prooftree}
				\]
				\[
				\begin{prooftree}
				\hypo{A, Γ ⊢ }
				\infer1{Γ ⊢ ¬_{L} A}
				\end{prooftree}
				\quad
				\begin{prooftree}
				\hypo{ ⊢ A, Δ}
				\infer1{¬_{L} A ⊢ Δ}
				\end{prooftree}
				\]
				
				NANDs and NORs
				
				\[
				\begin{prooftree}
				\hypo{⊢ A, Δ}
				\hypo{⊢ B, Δ}
				\infer2{¬A ⊕ ¬B ⊢ Δ}
				\end{prooftree}
				\quad
				\begin{prooftree}
				\hypo{Γ, A ⊢ }
				\infer1{Γ ⊢ ¬A ⊕ ¬B}
				\end{prooftree}
				\quad
				\begin{prooftree}
				\hypo{Γ, B ⊢ }
				\infer1{Γ ⊢ ¬A ⊕ ¬B}
				\end{prooftree}
				\]
				
				\[
				\begin{prooftree}
				\hypo{⊢ B, Δ}
				\hypo{ ⊢ A, Δ}
				\infer2{¬B ⊕ ¬A ⊢ Δ}
				\end{prooftree}
				\quad
				\begin{prooftree}
				\hypo{Γ, A ⊢ }
				\infer1{Γ ⊢ ¬B ⊕ ¬A}
				\end{prooftree}
				\quad
				\begin{prooftree}
				\hypo{Γ, B ⊢ }
				\infer1{Γ ⊢ ¬B ⊕ ¬A}
				\end{prooftree}
				\]
				
				\[
				\begin{prooftree}
				\hypo{ ⊢ A, Δ}
				\infer1{¬A \& ¬B ⊢ Δ}
				\end{prooftree}
				\quad
				\begin{prooftree}
				\hypo{ ⊢ B, Δ}
				\infer1{¬A \& ¬B ⊢ Δ}
				\end{prooftree}
				\quad
				\begin{prooftree}
				\hypo{Γ,A ⊢ }
				\hypo{Γ,B ⊢ }
				\infer2{Γ⊢ ¬A \& ¬B}
				\end{prooftree}
				\]
				
				\[
				\begin{prooftree}
				\hypo{ ⊢ A,Δ}
				\infer1{¬B \& ¬A ⊢ Δ}
				\end{prooftree}
				\quad
				\begin{prooftree}
				\hypo{ ⊢ B,Δ}
				\infer1{¬B \& ¬A ⊢ Δ}
				\end{prooftree}
				\quad
				\begin{prooftree}
				\hypo{Γ, B ⊢ }
				\hypo{Γ, A ⊢ }
				\infer2{Γ ⊢ ¬ B \& ¬ A}
				\end{prooftree}
				\]
				
				Conditionals
				
				\[
				\begin{prooftree}
				\hypo{⊢ B,Δ}
				\hypo{A ⊢ Δ}
				\infer2{¬B ⊕ A ⊢ Δ}
				\end{prooftree}
				\quad
				\begin{prooftree}
				\hypo{A ⊢ Δ}
				\hypo{⊢ B,Δ}
				\infer2{A ⊕ ¬B ⊢Δ}
				\end{prooftree}
				\quad
				\begin{prooftree}
				\hypo{Γ ⊢ A, Δ}
				\infer1{Γ ⊢ A ⊕ ¬B, Δ}
				\end{prooftree}
				\quad
				\begin{prooftree}
				\hypo{Γ, B ⊢ }
				\infer1{Γ ⊢ A ⊕ ¬B}
				\end{prooftree}
				\]
				
				\[
				\begin{prooftree}
				\hypo{ ⊢ A, Δ}
				\hypo{B ⊢ Δ}
				\infer2{¬A ⊕ B ⊢ Δ}
				\end{prooftree}
				\quad
				\begin{prooftree}
				\hypo{B ⊢ Δ}
				\hypo{ ⊢ A, Δ}
				\infer2{B ⊕ ¬A ⊢ Δ}
				\end{prooftree}
				\quad
				\begin{prooftree}
				\hypo{Γ, A ⊢ }
				\infer1{Γ ⊢ B ⊕ ¬A}
				\end{prooftree}
				\quad
				\begin{prooftree}
				\hypo{Γ ⊢ B, Δ}
				\infer1{Γ ⊢ B ⊕ ¬A, Δ}
				\end{prooftree}
				\]
				
				\[
				\begin{prooftree}
				\hypo{Γ, A ⊢ Δ}
				\infer1{Γ, A \& ¬B ⊢ Δ}
				\end{prooftree}
				\quad
				\begin{prooftree}
				\hypo{ ⊢ B, Δ}
				\infer1{A \& ¬B ⊢ Δ}
				\end{prooftree}
				\quad
				\begin{prooftree}
				\hypo{Γ⊢ A}
				\hypo{Γ,B ⊢ }
				\infer2{Γ⊢ A \& ¬B}
				\end{prooftree}
				\quad
				\begin{prooftree}
				\hypo{Γ,B ⊢ }
				\hypo{Γ⊢ A}
				\infer2{Γ⊢ ¬B \& A}
				\end{prooftree}
				\]
				
				\[
				\begin{prooftree}
				\hypo{ ⊢ A, Δ}
				\infer1{B \& ¬A ⊢ Δ}
				\end{prooftree}
				\quad
				\begin{prooftree}
				\hypo{Γ, B ⊢ Δ}
				\infer1{Γ, B \& ¬A ⊢ Δ}
				\end{prooftree}
				\quad
				\begin{prooftree}
				\hypo{Γ ⊢ B}
				\hypo{Γ,A ⊢ }
				\infer2{Γ ⊢ B \& ¬ A}
				\end{prooftree}
				\quad
				\begin{prooftree}
				\hypo{Γ,A ⊢ }
				\hypo{Γ ⊢ B}
				\infer2{Γ ⊢ ¬A \& B}
				\end{prooftree}
				\]
				
				Conjunction and Disjunction
				
				\[
				\begin{prooftree}
				\hypo{A ⊢ Δ}
				\hypo{B ⊢ Δ}
				\infer2{A ⊕ B ⊢ Δ}
				\end{prooftree}
				\quad
				\begin{prooftree}
				\hypo{Γ ⊢ A}
				\infer1{Γ ⊢ A ⊕ B}
				\end{prooftree}
				\quad
				\begin{prooftree}
				\hypo{Γ ⊢ B}
				\infer1{Γ ⊢ A ⊕ B}
				\end{prooftree}
				\]
				
				\[
				\begin{prooftree}
				\hypo{B ⊢ Δ}
				\hypo{A ⊢ Δ}
				\infer2{B ⊕ A ⊢ Δ}
				\end{prooftree}
				\quad
				\begin{prooftree}
				\hypo{Γ ⊢ A}
				\infer1{Γ ⊢ B ⊕ A}
				\end{prooftree}
				\quad
				\begin{prooftree}
				\hypo{Γ ⊢ B}
				\infer1{Γ ⊢ B ⊕ A}
				\end{prooftree}
				\]
				
				\[
				\begin{prooftree}
				\hypo{A ⊢ Δ}
				\infer1{A \& B ⊢ Δ}
				\end{prooftree}
				\quad
				\begin{prooftree}
				\hypo{B ⊢ Δ}
				\infer1{A \& B ⊢ Δ}
				\end{prooftree}
				\quad
				\begin{prooftree}
				\hypo{Γ ⊢ A}
				\hypo{Γ ⊢ B}
				\infer2{Γ ⊢ A \& B}
				\end{prooftree}
				\]
				
				\[
				\begin{prooftree}
				\hypo{A ⊢ Δ}
				\infer1{B \& A ⊢ Δ}
				\end{prooftree}
				\quad
				\begin{prooftree}
				\hypo{B ⊢ Δ}
				\infer1{B \& A ⊢ Δ}
				\end{prooftree}
				\quad
				\begin{prooftree}
				\hypo{Γ ⊢ B}
				\hypo{Γ ⊢ A}
				\infer2{Γ ⊢ B \& A}
				\end{prooftree}
				\]
				Biconditionals
				\[
				\begin{prooftree}
				\hypo{⊢ A, Δ}
				\hypo{B ⊢ Δ}
				\infer2{(¬A ⊕ B) \& (¬B ⊕ A) ⊢ Δ}
				\end{prooftree}
				\quad
				\begin{prooftree}
				\hypo{⊢ B, Δ}
				\hypo{A ⊢ Δ}
				\infer2{(¬A ⊕ B) \& (¬B ⊕ A) ⊢ Δ}
				\end{prooftree}
				\quad
				\begin{prooftree}
				\hypo{Γ, A ⊢ }
				\hypo{Γ, B ⊢ }
				\infer2{Γ ⊢ (¬A ⊕ B) \& (¬B ⊕ A)}
				\end{prooftree}
				\quad
				\begin{prooftree}
				\hypo{Γ ⊢ B, Δ}
				\hypo{Γ ⊢ A, Δ}
				\infer2{Γ ⊢ (¬A ⊕ B) \& (¬B ⊕ A), Δ}
				\end{prooftree}
				\]
				
				\[
				\begin{prooftree}
				\hypo{A ⊢ Δ}
				\hypo{⊢A, Δ}
				\infer2{(A \& B) ⊕  (¬A \& ¬B) ⊢ Δ}
				\end{prooftree}
				\quad
				\begin{prooftree}
				\hypo{A ⊢ Δ}
				\hypo{⊢B, Δ}
				\infer2{(A \& B) ⊕  (¬A \& ¬B) ⊢ Δ}
				\end{prooftree}
				\quad
				\begin{prooftree}
				\hypo{B ⊢ Δ}
				\hypo{⊢A, Δ}
				\infer2{(A \& B) ⊕  (¬A \& ¬B) ⊢ Δ}
				\end{prooftree}
				\quad
				\begin{prooftree}
				\hypo{B ⊢ Δ}
				\hypo{⊢B, Δ}
				\infer2{(A \& B) ⊕  (¬A \& ¬B) ⊢ Δ}
				\end{prooftree}
				\]
				
				\[
				\quad
				\begin{prooftree}
				\hypo{Γ ⊢ A, Δ}
				\hypo{Γ ⊢ B, Δ}
				\infer2{Γ ⊢ (A \& B) ⊕  (¬A \& ¬B),Δ}
				\end{prooftree}
				\quad
				\begin{prooftree}
				\hypo{Γ, B ⊢ }
				\hypo{Γ, A ⊢ }
				\infer2{Γ ⊢ (A \& B) ⊕  (¬A \& ¬B)}
				\end{prooftree}
				\]
				
				TODO: Apartness
				
			\end{center}
		
		\part{Theorems}
			\begin{center}
			\end{center}
	\end{center}


\end{document}
