
\documentclass{article}

\usepackage{amsmath}
\usepackage{ebproof}
\usepackage{fullpage}
\usepackage[utf8]{inputenc}
\usepackage{newunicodechar}
\usepackage{stix}

\newunicodechar{Γ}{\Gamma}
\newunicodechar{Δ}{\Delta}
\newunicodechar{Π}{\Pi}
\newunicodechar{Λ}{\Lambda}
\newunicodechar{Θ}{\Theta}

\newunicodechar{⊢}{\vdash}

\newunicodechar{℘}{\wp}
\newunicodechar{⊗}{\otimes}
\newunicodechar{⊕}{\oplus}
\newunicodechar{¬}{\neg}

\newunicodechar{→}{\rightarrow}

\newunicodechar{⊥}{\bot}
\newunicodechar{⊤}{\top}

\setlength{\parindent}{0em}

\author{James Martin, Ian D.L.N. Mclean}
\title{Ordinary Monotonic Disjunction Sequent Calculus}

\begin{document}

\maketitle

\begin{abstract}

\end{abstract}

\section{Structural Rules}

\begin{center}
	\[
	\begin{prooftree}
	\infer0[Id]{A ⊢ A}
	\end{prooftree}
	\]
	
	\[
	\begin{prooftree}
	\hypo{Γ ⊢ A}
	\hypo{A ⊢ Δ}
	\infer2[cut]{Γ ⊢ Δ}
	\end{prooftree}
	\]
\end{center}

\section{Unit Rules}
\begin{center}
	\[
	\begin{prooftree}
	\infer0{0 ⊢ A}
	\end{prooftree}
	\quad
	\begin{prooftree}
	\infer0{A ⊢ ⊤}
	\end{prooftree}
	\]
\end{center}

\section{Operational Rules}
\begin{center}
	\subsection{Additives}
	\begin{center}
		\[
		\begin{prooftree}
		\hypo{A ⊢ Δ}
		\hypo{B ⊢ Δ}
		\infer2{A ⊕ B ⊢ Δ}
		\end{prooftree}
		\quad
		\begin{prooftree}
		\hypo{Γ ⊢ A}
		\infer1{Γ ⊢ A ⊕ B}
		\end{prooftree}
		\quad
		\begin{prooftree}
		\hypo{Γ ⊢ B}
		\infer1{Γ ⊢ A ⊕ B}
		\end{prooftree}
		\]
		
		\[
		\begin{prooftree}
		\hypo{B ⊢ Δ}
		\hypo{A ⊢ Δ}
		\infer2{B ⊕ A ⊢ Δ}
		\end{prooftree}
		\quad
		\begin{prooftree}
		\hypo{Γ ⊢ A}
		\infer1{Γ ⊢ B ⊕ A}
		\end{prooftree}
		\quad
		\begin{prooftree}
		\hypo{Γ ⊢ B}
		\infer1{Γ ⊢ B ⊕ A}
		\end{prooftree}
		\]
	\end{center}
\end{center}

\part{Theorems}
	\begin{center}

		\[
		\begin{prooftree}
		\infer0{ ⊢ A ⊕ ¬A}
		\end{prooftree}
		\quad
		\begin{prooftree}
		\infer0{ ⊢ ¬A ⊕ A}
		\end{prooftree}
		\quad
		\begin{prooftree}
		\infer0{A \& ¬A ⊢ }
		\end{prooftree}
		\quad
		\begin{prooftree}
		\infer0{¬A \& A ⊢ }
		\end{prooftree}
		\]
		
		\[
		\begin{prooftree}
		\infer0{0 ⊢ C}
		\infer1{0 \& ¬ A ⊢ C}
		\end{prooftree}
		\quad
		\begin{prooftree}
		\infer0{C ⊢ ⊤}
		\infer1{C ⊢ ⊤ ⊕ ¬ A}
		\end{prooftree}		
		\]
		
		\[
		\begin{prooftree}
		\infer0{0 ⊢ A}
		\infer1{0 ⊢ A ⊕ ¬ A}
		\end{prooftree}
		\quad
		\begin{prooftree}
		\infer0{0 ⊢ ¬ A}
		\infer1{0 ⊢ A ⊕ ¬ A}
		\end{prooftree}
		\quad
		\begin{prooftree}
		\infer0{0 ⊢ }
		\infer1{⊢ A ⊕ ¬ 0}
		\end{prooftree}
		\quad
		\begin{prooftree}
		\infer0{C ⊢ ⊤}
		\infer1{C ⊢ ⊤ ⊕ A}
		\end{prooftree}
		\]
		
		\[
		\begin{prooftree}
		\infer0{A ⊢ ⊤}
		\infer1{A \& ¬ A ⊢ ⊤}
		\end{prooftree}
		\quad
		\begin{prooftree}
		\infer0{¬ A ⊢ ⊤}
		\infer1{A \& ¬ A ⊢ ⊤}
		\end{prooftree}
		\]
		
		\[
		\begin{prooftree}
		\infer0{1 ⊢ 1}
		\infer1{1 ⊢ 1 ⊕ ¬ 1}
		\end{prooftree}
		\quad
		\begin{prooftree}
		\infer0{0 ⊢ 1 ⊕ ¬ 1}
		\end{prooftree}
		\quad
		\begin{prooftree}
		\hypo{⊥ ⊢ 1 ⊕ ¬ 1}
		\end{prooftree}
		\quad
		\begin{prooftree}
		\hypo{⊤ ⊢ 1 ⊕ ¬ 1}
		\end{prooftree}
		\]
		
		\[
		\begin{prooftree}
		\infer0{⊥⊢}
		\infer1{⊢ ¬ ⊥}
		\infer1{⊢ ⊥ ⊕ ¬ ⊥}
		\infer1{1 ⊢ ⊥ ⊕ ¬ ⊥}
		\end{prooftree}
		\quad
		\begin{prooftree}
		\infer0{0 ⊢ ⊥ ⊕ ¬ ⊥}
		\end{prooftree}
		\quad
		\begin{prooftree}
		\infer0{⊥ ⊢ ⊥}
		\infer1{⊥ ⊢ ⊥ ⊕ ¬ ⊥}
		\end{prooftree}
		\quad
		\begin{prooftree}
		\hypo{⊤ ⊢ ⊥ ⊕ ¬ ⊥}
		\end{prooftree}
		\]
		
		\[
		\begin{prooftree}
		\infer0{0 ⊢}
		\infer1{⊢ ¬ 0}
		\infer1{⊢ 0 ⊕ ¬ 0}
		\infer1{1 ⊢ 0 ⊕ ¬ 0}
		\end{prooftree}
		\quad
		\begin{prooftree}
		\infer0{0 ⊢ 0 ⊕ ¬ 0}
		\end{prooftree}
		\quad
		\begin{prooftree}
		\hypo{⊥ ⊢ 0 ⊕ ¬ 0}
		\end{prooftree}
		\quad
		\begin{prooftree}
		\hypo{⊤ ⊢ 0 ⊕ ¬ 0}
		\end{prooftree}
		\]
		
		\[
		\begin{prooftree}
		\infer0{⊢ ⊤}
		\infer1{⊢ ⊤ ⊕ ¬ ⊤}
		\infer1{1 ⊢ ⊤ ⊕ ¬ ⊤}
		\end{prooftree}
		\quad
		\begin{prooftree}
		\infer0{0 ⊢ ⊤ ⊕ ¬ ⊤}
		\end{prooftree}
		\quad
		\begin{prooftree}
		\infer0{⊥ ⊢ ⊤}
		\infer1{⊥ ⊢ ⊤ ⊕ ¬ ⊤}
		\end{prooftree}
		\quad
		\begin{prooftree}
		\infer0{⊤ ⊢ ⊤}
		\infer1{⊤ ⊢ ⊤ ⊕ ¬ ⊤}
		\end{prooftree}
		\]
		
		\[
		\begin{prooftree}
		\infer0{1 ⊢ 1}
		\infer1{1 \&  ¬ 1⊢ 1}
		\end{prooftree}
		\quad
		\begin{prooftree}
		\hypo{1 \&  ¬ 1⊢ 0}
		\end{prooftree}
		\quad
		\begin{prooftree}
		\infer0{⊢ 1}
		\infer1{¬ 1⊢ }
		\infer1{1 \&  ¬ 1⊢ }
		\infer1{1 \&  ¬ 1⊢ ⊥}
		\end{prooftree}
		\quad
		\begin{prooftree}
		\infer0{1 \&  ¬ 1 ⊢ ⊤}
		\end{prooftree}
		\]
		
		\[
		\begin{prooftree}
		\infer0{0 ⊢ 1}
		\infer1{0 \&  ¬ 0 ⊢ 1}
		\end{prooftree}
		\quad
		\begin{prooftree}
		\infer0{0 ⊢ 0}
		\infer1{0 \&  ¬ 0 ⊢ 0}
		\end{prooftree}
		\quad
		\begin{prooftree}
		\infer0{0 ⊢ ⊥}
		\infer1{0 \&  ¬ 0 ⊢ ⊥}
		\end{prooftree}
		\quad
		\begin{prooftree}
		\infer0{0 \&  ¬ 0 ⊢ ⊤}
		\end{prooftree}
		\]
		
		\[
		\begin{prooftree}
		\hypo{⊥ \&  ¬ ⊥ ⊢ 1}
		\end{prooftree}
		\quad
		\begin{prooftree}
		\hypo{⊥ \&  ¬ ⊥ ⊢ 0}
		\end{prooftree}
		\quad
		\begin{prooftree}
		\infer0{⊥ ⊢ }
		\infer1{⊥ \&  ¬ ⊥ ⊢ }
		\infer1{⊥ \&  ¬ ⊥ ⊢ ⊥}
		\end{prooftree}
		\quad
		\begin{prooftree}
		\infer0{⊥ \&  ¬ ⊥ ⊢ ⊤}
		\end{prooftree}
		\]
		
		\[
		\begin{prooftree}
		\hypo{⊤ \&  ¬ ⊤ ⊢ 1}
		\end{prooftree}
		\quad
		\begin{prooftree}
		\hypo{⊤ \&  ¬ ⊤ ⊢ 0}
		\end{prooftree}
		\quad
		\begin{prooftree}
		\infer0{⊢ ⊤}
		\infer1{¬ ⊤ ⊢}
		\infer1{¬ ⊤ ⊢ ⊥}
		\infer1{⊤ \&  ¬ ⊤ ⊢ ⊥}
		\end{prooftree}
		\quad
		\begin{prooftree}
		\infer0{⊤ \&  ¬ ⊤ ⊢ ⊤}
		\end{prooftree}
		\]
	\end{center}

\end{document}
