\begin{equation*}\n\displaystyle \begin{array}{lll}\\
 \displaystyle  \partial M = \frac{\kappa}{8 \pi} \partial A + \Omega \partial J + \Phi \partial Q \\\\
 \displaystyle  \partial M = 0 \text{ and } \partial A = 0, \partial J = - \frac{\Phi \partial Q}{\Omega} \\\\
 \displaystyle  \partial M = 0 \text{ and } \partial A = 0, \partial Q = - \frac{\Omega \partial J}{\Phi} \\\\
 \displaystyle  \partial M = 0, \partial J = -\frac{(\frac{\kappa}{8 \pi} \partial A + \Phi \partial Q)}{\Omega} \\\\
 \displaystyle  \partial M = 0, \partial Q = -\frac{(\frac{\kappa}{8 \pi} \partial A + \Omega \partial J)}{\Phi}  \\\\

\end{array}

\displaystyle \begin{array}{lll}\\
 \displaystyle  \partial M = \frac{\kappa}{8 \pi} \partial A + \Omega \partial J + \Phi \partial Q \\\\
 \displaystyle  0 = \frac{\kappa}{8 \pi} \partial A + \Omega \partial J + \Phi \partial Q - \partial M \\\\
 \displaystyle  \frac{\kappa}{8 \pi} \partial A = \partial M - \Omega \partial J - \Phi \partial Q \\\\
 \displaystyle  \Phi \partial Q = \partial M - \frac{\kappa}{8 \pi} \partial A - \Omega \partial J \\\\
 \displaystyle  \Omega \partial J = \partial M - \frac{\kappa}{8 \pi} \partial A - \Phi \partial Q \\\\

\end{array}

\displaystyle \begin{array}{lll}\\
 \displaystyle  \partial M = \frac{\kappa}{8 \pi} \partial A + \Omega \partial J + \Phi \partial Q \\\\
 \displaystyle  0 = \frac{\kappa}{8 \pi} \partial A + \Omega \partial J + \Phi \partial Q - \partial M \\\\
 \displaystyle  \frac{\kappa}{8 \pi} \partial A = \partial M - \Omega \partial J - \Phi \partial Q \\\\
 \displaystyle  \partial A = \frac{8 \pi(\partial M - \Omega \partial J - \Phi \partial Q)}{\kappa}\\\\

 \displaystyle  \Phi \partial Q = \partial M - \frac{\kappa}{8 \pi} \partial A - \Omega \partial J \\\\
 \displaystyle  \partial Q = \frac{\partial M - \frac{\kappa}{8 \pi} \partial A - \Omega \partial J}{\Phi} \\\\

 \displaystyle  \Omega \partial J = \partial M - \frac{\kappa}{8 \pi} \partial A - \Phi \partial Q \\\\
 \displaystyle  \partial J = \frac{\partial M - \frac{\kappa}{8 \pi} \partial A - \Phi \partial Q}{\Omega} \\\\

\end{array}

\displaystyle \begin{array}{lll}\\
 \displaystyle  \partial M = \frac{\kappa}{8 \pi} \partial A + \Omega \partial J + \Phi \partial Q \\\\
 \displaystyle  \partial A = \frac{8 \pi(\partial M - \Omega \partial J - \Phi \partial Q)}{\kappa}\\\\

 \displaystyle  \partial M - \partial A = \frac{\kappa}{8 \pi} \partial A + \Omega \partial J + \Phi \partial Q - \frac{8 \pi(\partial M - \Omega \partial J - \Phi \partial Q)}{\kappa}\\\\
 \displaystyle  \partial M - \partial A = \frac{\kappa}{8 \pi} \partial A + \Omega \partial J + \Phi \partial Q - (\frac{8 \pi \partial M}{\kappa} - \frac{8 \pi \Omega \partial J}{\kappa} - \frac{8 \pi \Phi \partial Q}{\kappa})\\\\
 \displaystyle  \partial M - \partial A = \frac{\kappa}{8 \pi} \partial A + \Omega \partial J + \Phi \partial Q - \frac{8 \pi \partial M}{\kappa} + \frac{8 \pi \Omega \partial J}{\kappa} + \frac{8 \pi \Phi \partial Q}{\kappa}\\\\
 \displaystyle  \partial M + \frac{8 \pi \partial M}{\kappa} - (\partial A + \frac{\kappa}{8 \pi} \partial A) = \Omega \partial J + \frac{8 \pi \Omega \partial J}{\kappa} + \Phi \partial Q + \frac{8 \pi \Phi \partial Q}{\kappa}\\\\

\end{array}

\displaystyle \begin{array}{lll}\\
 \displaystyle  0 = \frac{\kappa}{8 \pi} \partial A + \Omega \partial J + \Phi \partial Q - \partial M \\\\

 \displaystyle  \partial M = \frac{\kappa}{8 \pi} \partial A + \Omega \partial J + \Phi \partial Q \\\\


 \displaystyle  \partial A = \frac{8 \pi\partial M}{\kappa} - \frac{8 \pi \Omega \partial J}{\kappa} - \frac{8 \pi \Phi \partial Q}{\kappa}\\\\

 \displaystyle  \partial Q = \frac{\partial M}{\Phi} - \frac{\kappa}{8 \pi} \frac{ \partial A}{\Phi} - \frac{\Omega \partial J}{\Phi} \\\\

 \displaystyle  \partial J = \frac{\partial M}{\Omega} - \frac{\kappa}{8 \pi} \frac{ \partial A}{\Omega} - \frac{\Phi \partial Q}{\Omega} \\\\

\end{array}

\displaystyle \begin{array}{lll}\\
 \displaystyle \frac{\kappa}{8 \pi} \partial A + \Omega \partial J + \Phi \partial Q - \partial M = 0 \\\\

\begin{bmatrix} 
\partial M \\
\partial A \\
\partial J \\
\partial Q \\
\end{bmatrix}
=
\begin{bmatrix} 
1\\
\frac{8 \pi}{\kappa}\\
\frac{1}{\Omega}\\
\frac{1}{\Phi}\\
\end{bmatrix}

\begin{bmatrix} 
0 & \frac{\kappa}{8 \pi} \partial A & \Omega \partial J & \Phi \partial Q\\
\partial M & 0 & - \Omega \partial J & - \Phi \partial Q\\
\partial M & - \frac{\kappa}{8 \pi} \partial A & 0 & - \Phi \partial Q\\
\partial M & - \frac{\kappa}{8 \pi} \partial A & - \Omega \partial J & 0\\
\end{bmatrix}


\end{array}\n\end{equation*}
