}

\maketitle

\begin{abstract}
A sequent system defined by the absence of non-contradiction, excluded middle, logical explosion, and logical implosion in the presence of structural rules.
\end{abstract}

\section{Structural Rules}

\begin{center}
	\[
	\begin{prooftree}
	\infer0[Id]{A ⊢ A}
	\end{prooftree}
	\]
	
	\[
	\begin{prooftree}
	\hypo{Γ ⊢ A}
	\hypo{A ⊢ Δ}
	\infer2[Cut]{Γ ⊢ Δ}
	\end{prooftree}
	\]
\end{center}

\section{Unit Rules}
\begin{center}
		\[
	\begin{prooftree}
	\hypo{Γ_{L}, Γ_{R} ⊢ C}
	\infer1{Γ_{L}, 1, Γ_{R} ⊢ C}
	\end{prooftree}
	\quad
	\begin{prooftree}
	\hypo{C ⊢ Δ_{L}, Δ_{R}}
	\infer1{C ⊢ Δ_{L}, ⊥, Δ_{R}}
	\end{prooftree}
	\]
	
	\[
	\begin{prooftree}
	\infer0{ ⊥ ⊢ }
	\end{prooftree}
	\quad
	\begin{prooftree}
	\infer0{ ⊢ 1}
	\end{prooftree}
	\]
	
	\[
	\begin{prooftree}
	\infer0{ 0 ⊢ Δ}
	\end{prooftree}
	\quad
	\begin{prooftree}
	\infer0{ Γ ⊢ ⊤}
	\end{prooftree}
	\]
\end{center}

\section{Operational Rules}
\begin{center}
	\subsection{Negations}
	\begin{center}
		\[
		\begin{prooftree}
		\hypo{⊢ A}
		\infer1{¬ A ⊢ }
		\end{prooftree}
		\quad
		\begin{prooftree}
		\hypo{ A ⊢ }
		\infer1{ ⊢ ¬ A}
		\end{prooftree}
		\]
	\end{center}

	\subsection{Additives}
	\begin{center}
		\[
		\begin{prooftree}
		\hypo{A ⊢ Δ}
		\hypo{B ⊢ Δ}
		\infer2{A ⅋ B ⊢ Δ}
		\end{prooftree}
		\quad
		\begin{prooftree}
		\hypo{Γ ⊢ A, B }
		\infer1{Γ ⊢ A ⅋ B}
		\end{prooftree}
		\]
		
		\[
		\begin{prooftree}
		\hypo{Γ, A, Φ ⊢ Ψ}
		\infer1{Γ, A \& B, Φ ⊢ Ψ}
		\end{prooftree}
		\quad
		\begin{prooftree}
		\hypo{Γ, B, Φ ⊢ Ψ}
		\infer1{Γ, A \& B, Φ ⊢ Ψ}
		\end{prooftree}
		\quad
		\begin{prooftree}
		\hypo{ Γ ⊢ Δ, B, Ψ}
		\hypo{ Γ ⊢ Δ, A, Ψ}
		\infer2{ Γ ⊢ Δ, B \& A, Ψ}
		\end{prooftree}
		\]
		
		\[
		\begin{prooftree}
		\hypo{Γ, A, Φ ⊢ C}
		\hypo{Γ, B, Φ ⊢ C}
		\infer2{Γ, A ⊕ B, Φ ⊢ C}
		\end{prooftree}
		\quad
		\begin{prooftree}
		\hypo{Γ ⊢ A}
		\infer1{Γ ⊢ A ⊕ B}
		\end{prooftree}
		\quad
		\begin{prooftree}
		\hypo{Γ ⊢ B}
		\infer1{Γ ⊢ A ⊕ B}
		\end{prooftree}
		\quad
		\begin{prooftree}
		\hypo{A ⊢ Δ}
		\infer1{A \& B ⊢ Δ}
		\end{prooftree}
		\quad
		\begin{prooftree}
		\hypo{B ⊢ Δ}
		\infer1{A \& B ⊢ Δ}
		\end{prooftree}
		\quad
		\begin{prooftree}
		\hypo{ C ⊢ Ψ, B, Δ}
		\hypo{ C ⊢ Ψ, A, Δ}
		\infer2{ C ⊢ Ψ, B \& A, Δ}
		\end{prooftree}
		\]
		
		\[
		\begin{prooftree}
		\hypo{Γ, A, Φ ⊢ C}
		\infer1{Γ, A \& B, Φ ⊢ C}
		\end{prooftree}
		\quad
		\begin{prooftree}
		\hypo{Γ, B, Φ ⊢ C}
		\infer1{Γ, A \& B, Φ ⊢ C}
		\end{prooftree}
		\quad
		\begin{prooftree}
		\hypo{Γ ⊢ A}
		\hypo{Γ ⊢ B}
		\infer2{Γ ⊢ A \& B}
		\end{prooftree}
		\quad
		\begin{prooftree}
		\hypo{B ⊢ Δ}
		\hypo{A ⊢ Δ}
		\infer2{B ⊕ A ⊢ Δ}
		\end{prooftree}
		\quad
		\begin{prooftree}
		\hypo{C ⊢ Ψ, A, Δ}
		\infer1{C ⊢ Ψ, B ⊕ A, Δ}
		\end{prooftree}
		\quad
		\begin{prooftree}
		\hypo{C ⊢ Ψ, B, Δ}
		\infer1{C ⊢ Ψ, B ⊕ A, Δ}
		\end{prooftree}
		\]
		
		
		\[
		\begin{prooftree}
		\hypo{Γ, Φ ⊢ C, A}
		\hypo{Γ, Φ ⊢ C, B}
		\infer2{Γ, ¬ A ⊕ ¬ B, Φ ⊢ C}
		\end{prooftree}
		\quad
		\begin{prooftree}
		\hypo{A, Γ ⊢ }
		\infer1{Γ ⊢ ¬ A ⊕ ¬ B}
		\end{prooftree}
		\quad
		\begin{prooftree}
		\hypo{B, Γ ⊢ }
		\infer1{Γ ⊢ ¬ A ⊕ ¬ B}
		\end{prooftree}
		\quad
		\begin{prooftree}
		\hypo{⊢ Δ, A}
		\infer1{¬ B \& ¬ A ⊢ Δ}
		\end{prooftree}
		\quad
		\begin{prooftree}
		\hypo{⊢ Δ, B}
		\infer1{¬ B \& ¬ A ⊢ Δ}
		\end{prooftree}
		\quad
		\begin{prooftree}
		\hypo{ B, C ⊢ Ψ, Δ}
		\hypo{ A, C ⊢ Ψ, Δ}
		\infer2{ C ⊢ Ψ, ¬ B \& ¬ A, Δ}
		\end{prooftree}
		\]
		
		\[
		\begin{prooftree}
		\hypo{Γ, Φ ⊢ C, A}
		\infer1{Γ, ¬ A \& ¬ B, Φ ⊢ C}
		\end{prooftree}
		\quad
		\begin{prooftree}
		\hypo{Γ, Φ ⊢ C, B}
		\infer1{Γ, ¬ A \& ¬ B, Φ ⊢ C}
		\end{prooftree}
		\quad
		\begin{prooftree}
		\hypo{A, Γ ⊢ }
		\hypo{B, Γ ⊢ }
		\infer2{Γ ⊢ ¬ A \& ¬ B}
		\end{prooftree}
		\quad
		\begin{prooftree}
		\hypo{⊢ Δ, B}
		\hypo{⊢ Δ, A}
		\infer2{¬ B ⊕ ¬ A ⊢ Δ}
		\end{prooftree}
		\quad
		\begin{prooftree}
		\hypo{A, C ⊢ Ψ, Δ}
		\infer1{C ⊢ Ψ, ¬ B ⊕ ¬ A, Δ}
		\end{prooftree}
		\quad
		\begin{prooftree}
		\hypo{B, C ⊢ Ψ, Δ}
		\infer1{C ⊢ Ψ, ¬ B ⊕ ¬ A, Δ}
		\end{prooftree}
		\]
		
	\end{center}

	\subsection{Multiplicatives}
	\begin{center}
		\[
		\begin{prooftree}
		\hypo{Γ, A, B, Φ ⊢ C}
		\infer1{Γ, A ⊗ B, Φ ⊢ C}
		\end{prooftree}
		\quad
		\begin{prooftree}
		\hypo{Γ ⊢ A}
		\hypo{Φ ⊢ B}
		\infer2{Γ, Φ ⊢ A ⊗ B}
		\end{prooftree}
		\quad
		\begin{prooftree}
		\hypo{B ⊢ Ψ}
		\hypo{A ⊢ Δ}
		\infer2{B ⅋ A ⊢ Ψ, Δ}
		\end{prooftree}
		\quad
		\begin{prooftree}
		\hypo{C ⊢ Ψ, B, A, Δ}
		\infer1{C ⊢ Ψ, B ⅋ A, Δ}
		\end{prooftree}
		\]
		
		\[
		\begin{prooftree}
		\hypo{Γ, B, A, Φ ⊢ C}
		\infer1{Γ, B ⊗ A, Φ ⊢ C}
		\end{prooftree}
		\quad
		\begin{prooftree}
		\hypo{Φ ⊢ B}
		\hypo{Γ ⊢ A}
		\infer2{Φ, Γ ⊢ B ⊗ A}
		\end{prooftree}
		\quad
		\begin{prooftree}
		\hypo{A ⊢ Δ}
		\hypo{B ⊢ Ψ}
		\infer2{A ⅋ B ⊢ Δ, Ψ}
		\end{prooftree}
		\quad
		\begin{prooftree}
		\hypo{C ⊢ Ψ, A, B, Δ}
		\infer1{C ⊢ Ψ, A ⅋ B, Δ}
		\end{prooftree}
		\]
		
		\[
		\begin{prooftree}
		\hypo{Γ ⊢ A}
		\hypo{Φ, B, Θ ⊢ C}
		\infer2{Φ, Γ, A → B, Θ ⊢ C}
		\end{prooftree}
		\quad
		\begin{prooftree}
		\hypo{A, Γ ⊢ B}
		\infer1{Γ ⊢ A → B}
		\end{prooftree}
		\quad
		\begin{prooftree}
		\hypo{B ⊢ Δ, A}
		\infer1{A ↚ B ⊢ Δ}
		\end{prooftree}
		\quad
		\begin{prooftree}
		\hypo{A ⊢ Δ}
		\hypo{C ⊢ Λ, B, Ψ}
		\infer2{C ⊢ Λ, A ↚ B, Ψ, Δ}
		\end{prooftree}
		\]
		
		\[
		\begin{prooftree}
		\hypo{Γ ⊢ A}
		\hypo{Φ, B, Θ ⊢ C}
		\infer2{Φ, Γ, B ← A, Θ ⊢ C}
		\end{prooftree}
		\quad
		\begin{prooftree}
		\hypo{Γ, A ⊢ B}
		\infer1{Γ ⊢ B ← A}
		\end{prooftree}
		\quad
		\begin{prooftree}
		\hypo{B ⊢ A, Ψ}
		\infer1{A ↛ B ⊢ Ψ}
		\end{prooftree}
		\quad
		\begin{prooftree}
		\hypo{A ⊢ Δ}
		\hypo{C ⊢ Λ, B, Ψ}
		\infer2{C ⊢ Λ, B ↛ A, Ψ, Δ}
		\end{prooftree}
		\]
	\end{center}
\end{center}

\part{Theorems}
	\begin{center}
		\[
		\begin{prooftree}
		\infer0{A ⊢ A}
		\infer1{1, A ⊢ A}
		\infer1{1 ⊢ A, ¬ A}
		\infer1{1 ⊢ A ⅋ ¬ A}
		\end{prooftree}
		\quad
		\begin{prooftree}
		\infer0{A ⊢ A}
		\infer1{A, 1 ⊢ A}
		\infer1{A ⊗ 1 ⊢ A}
		\end{prooftree}
		\quad
		\begin{prooftree}
		\infer0{A, 0 ⊢ A}
		\infer1{A ⊗ 0 ⊢ A}
		\end{prooftree}
		\quad
		\begin{prooftree}
		\infer0{0 ⊢ A ⅋ ¬ A}
		\end{prooftree}
		\]
		
		\[
		\begin{prooftree}
		\infer0{A ⊢ A}
		\infer1{A ⊢ A, ⊥}
		\infer1{A, ¬ A ⊢ ⊥}
		\infer1{A ⊗ ¬ A ⊢ ⊥}
		\end{prooftree}
		\quad
		\begin{prooftree}
		\infer0{A ⊢ A}
		\infer1{A ⊢ A, ⊥}
		\infer1{A ⊢ A ⅋ ⊥}
		\end{prooftree}
		\quad
		\begin{prooftree}
		\infer0{A ⊢ A, ⊤}
		\infer1{A ⊢ A ⅋ ⊤}
		\end{prooftree}
		\quad
		\begin{prooftree}
		\infer0{A ⊗ ¬ A ⊢ ⊤}
		\end{prooftree}
		\]
		
		\[
		\begin{prooftree}
		\infer0{⊥ ⊢ }
		\infer1{⊥ ⊢ ⊥}
		\infer1{⊥, ¬ ⊥ ⊢ }
		\infer1{⊥ ⊗ ¬ ⊥ ⊢ }
		\end{prooftree}
		\quad
		\begin{prooftree}
		\infer0{A ⊢ A}
		\infer1{A ⊢ A, ⊥}
		\infer1{A, ¬ ⊥ ⊢ A}
		\infer1{A ⊗ ¬ ⊥ ⊢ A}
		\end{prooftree}
		\quad
		\begin{prooftree}
		\infer0{ ⊢ 1}
		\infer1{1 ⊢ 1}
		\infer1{1, ¬ 1 ⊢ }
		\infer1{1 ⊗ ¬ 1 ⊢ }
		\end{prooftree}
		\quad
		\begin{prooftree}
		\infer0{A ⊢ A}
		\infer1{A, 1 ⊢ A}
		\infer1{1, ¬ A ⊢ ¬ A}
		\infer1{1 ⊗ ¬ A ⊢ ¬ A}
		\end{prooftree}
		\quad
		\begin{prooftree}
		\infer0{0 ⊢ Δ, A}
		\infer1{0, ¬ A ⊢ Δ}
		\infer1{0 ⊗ ¬ A ⊢ Δ}
		\end{prooftree}
		\quad
		\begin{prooftree}
		\infer0{A ⊢ Δ, ⊤}
		\infer1{A, ¬ ⊤ ⊢ Δ}
		\infer1{A ⊗ ¬ ⊤ ⊢ Δ}
		\end{prooftree}
		\]
		
		\[
		\begin{prooftree}
		\infer0{A ⊢ A}
		\infer1{¬A ⊢ ¬A}
		\infer1{¬A ⊢ ¬A,  ⊥}
		\infer1{¬A ⊢ ¬A ⅋ ⊥}
		\end{prooftree}
		\quad
		\begin{prooftree}
		\infer0{A ⊢ A}
		\infer1{1, A ⊢ A}
		\infer1{A ⊢ A, ¬1}
		\infer1{A ⊢ A ⅋ ¬1}
		\end{prooftree}
		\quad
		\begin{prooftree}
		\infer0{0, Γ ⊢ A}
		\infer1{Γ ⊢ A, ¬0}
		\infer1{Γ ⊢ A ⅋ ¬0}
		\end{prooftree}
		\quad
		\begin{prooftree}
		\infer0{A, Γ ⊢ ⊤}
		\infer1{ Γ⊢ ⊤, ¬A}
		\infer1{Γ ⊢ ⊤ ⅋ ¬A}
		\end{prooftree}
		\]
		
		\[
		\begin{prooftree}
		\infer0{⊥ ⊢ }
		\infer1{⊥ ⊢ ⊥}
		\infer1{⊥, ¬ ⊥ ⊢ }
		\infer1{⊢ ⊥ ⅋ ¬ ⊥}
		\end{prooftree}
		\quad
		\begin{prooftree}
		\infer0{ ⊢ 1}
		\infer1{1 ⊢ 1}
		\infer1{1, ¬ 1 ⊢ }
		\infer1{1 ⊗ ¬ 1 ⊢ }
		\end{prooftree}
		\quad
		\begin{prooftree}
		\infer0{0 ⊢ Δ, A}
		\infer1{0, ¬ A ⊢ Δ}
		\infer1{0 ⊗ ¬ A ⊢ Δ}
		\end{prooftree}
		\quad
		\begin{prooftree}
		\infer0{A ⊢ Δ, ⊤}
		\infer1{A, ¬ ⊤ ⊢ Δ}
		\infer1{A ⊗ ¬ ⊤ ⊢ Δ}
		\end{prooftree}
		\]
		
		\[
		\begin{prooftree}
		\infer0{A ⊢ A}
		\infer1{A ⊢ A ⊕ ¬A}
		\end{prooftree}
		\quad
		\begin{prooftree}
		\infer0{A ⊢ A}
		\infer1{ ¬ A \& A ⊢ A}
		\end{prooftree}
		\]
		
		\[
		\begin{prooftree}
		\infer0{A ⊢ A}
		\infer1{¬ A, A ⊢}
		\infer1{ ¬ A ⊗ A ⊢}
		\end{prooftree}
		\quad
		\begin{prooftree}
		\infer0{A ⊢ A}
		\infer1{¬ A, A ⊢}
		\infer1{A ⊗ ¬ A ⊢}
		\infer1{⊢¬ (A ⊗ ¬ A)}
		\end{prooftree}
		\]

		\[
		\begin{prooftree}
		\infer0{A ⊢ A}
		\infer1{⊢ A, ¬ A}
		\infer1{⊢ A ⅋ ¬ A}
		\end{prooftree}
		\quad
		\begin{prooftree}
		\infer0{A ⊢ A}
		\infer1{⊢ A, ¬ A}
		\infer1{⊢ A ⅋ ¬ A}
		\infer1{¬ (A ⅋ ¬ A) ⊢}
		\end{prooftree}
		\]

		\[
		\begin{prooftree}
		\infer0{⊥ ⊢}
		\infer1{A \& ⊥ ⊢}
		\end{prooftree}
		\quad
		\begin{prooftree}
		\infer0{0 ⊢}
		\infer1{A \& 0 ⊢}
		\end{prooftree}
		\quad
		\begin{prooftree}
		\infer0{A ⊢ A}
		\infer0{A ⊢ ⊤}
		\infer2{A ⊢ A \& ⊤}
		\end{prooftree}
		\]
		
		\[
		\begin{prooftree}
		\infer0{⊢ 1}
		\infer1{⊢ A ⊕ 1}
		\end{prooftree}
		\quad
		\begin{prooftree}
		\infer0{⊢ ⊤}
		\infer1{⊢ A ⊕ ⊤}
		\end{prooftree}
		\quad
		\begin{prooftree}
		\infer0{A ⊢ A}
		\infer0{0 ⊢ A}
		\infer2{A ⊕ 0 ⊢ A}
		\end{prooftree}
		\]
	\end{center}

\end{document}}*}
