


\begin{abstract}
Strictly visible structural additive calculus with first order quantification.
\end{abstract}

\section{Structural Rules}

\begin{center}
	\[
	\begin{prooftree}
	\infer0[Id]{A $\vdash$  A}
	\end{prooftree}
	\]
	
	\[
	\begin{prooftree}
	\hypo{$\Gamma$  $\vdash$  A}
	\hypo{A $\vdash$  $\Delta$ }
	\infer2[Cut]{$\Gamma$  $\vdash$  $\Delta$ }
	\end{prooftree}
	\]
	
	\[
	\begin{prooftree}
	\hypo{$\vdash$  C}
	\infer1[wL]{A $\vdash$  C}
	\end{prooftree}
	\qquad
	\begin{prooftree}
	\hypo{C $\vdash$  }
	\infer1[Rw]{C $\vdash$  A}
	\end{prooftree}
	\]
	
	\[
	\begin{prooftree}
	\hypo{A, A $\vdash$  C}
	\infer1[cL]{A $\vdash$  C}
	\end{prooftree}
	\qquad
	\begin{prooftree}
	\hypo{C $\vdash$  A, A}
	\infer1[Rc]{C $\vdash$  A}
	\end{prooftree}
	\]
	
	\[
	\begin{prooftree}
	\hypo{A, B $\vdash$  C}
	\infer1[pL]{B, A $\vdash$  C}
	\end{prooftree}
	\qquad
	\begin{prooftree}
	\hypo{C $\vdash$  A, B}
	\infer1[Rp]{C $\vdash$  B, A}
	\end{prooftree}
	\]
\end{center}

\section{Units}
	\begin{center}
		\[
		\begin{prooftree}
		\infer0{\bot $\vdash$  $\Delta$ }
		\end{prooftree}
		\quad
		\begin{prooftree}
		\infer0{$\Gamma$  $\vdash$  \top}
		\end{prooftree}
		\]
	\end{center}

\section{Quantifiers}
	\begin{center}
		Standard Eigenvariable Condition Quantifiers
		\[
		\begin{prooftree}
		\hypo{P[t/x] $\vdash$  $\Delta$ }
		\infer1{$\forall$ x.P(x) $\vdash$  $\Delta$ }
		\end{prooftree}
		\quad
		\begin{prooftree}
		\hypo{$\Gamma$  $\vdash$  P[y/x]}
		\infer1{$\Gamma$  $\vdash$  $\forall$ x.P(x)}
		\end{prooftree}
		\]
		in $$\forall$ R$ the variable y must not occur free anywhere in the lower sequent.
		\[
		\begin{prooftree}
		\hypo{P[y/x] $\vdash$  $\Delta$ }
		\infer1{$\exists$ x.P(x) $\vdash$  $\Delta$ }
		\end{prooftree}
		\quad
		\begin{prooftree}
		\hypo{$\Gamma$  $\vdash$  P[t/x]}
		\infer1{$\Gamma$  $\vdash$  $\exists$ x.P(x)}
		\end{prooftree}
		\]
		in $$\exists$ L$ the variable y must not occur free anywhere in the lower sequent.
		\[
		\begin{prooftree}
		\hypo{P(y)$\vdash$ }
		\infer1{$\neg$ $\forall$ x.$\neg$ P(x) $\vdash$  }
		\end{prooftree}
		\quad
		\begin{prooftree}
		\hypo{$\vdash$ P(t)}
		\infer1{$\vdash$  $\neg$ $\forall$ x.$\neg$ P(x)}
		\end{prooftree}
		\quad
		\begin{prooftree}
		\hypo{P(t)$\vdash$ }
		\infer1{$\neg$ $\exists$ x.$\neg$ P(x) $\vdash$  }
		\end{prooftree}
		\quad
		\begin{prooftree}
		\hypo{$\vdash$ P(y)}
		\infer1{$\vdash$  $\neg$ $\exists$ x.$\neg$ P(x)}
		\end{prooftree}
		\]
		
		
		Henkin constant quantifiers
		\[
		\begin{prooftree}
		\hypo{P(t/x) $\vdash$  $\Delta$ }
		\infer1{$\forall$ xP(x) $\vdash$  $\Delta$ }
		\end{prooftree}
		\quad
		\begin{prooftree}
		\hypo{$\Gamma$  $\vdash$  P (c_{$\forall$ x.P}/x)}
		\infer1{$\Gamma$  $\vdash$  $\forall$ xP(x)}
		\end{prooftree}
		\]
		
		\[
		\begin{prooftree}
		\hypo{P(c_{$\exists$ x.P}/x) $\vdash$  $\Delta$ }
		\infer1{$\exists$ xP(x) $\vdash$  $\Delta$ }
		\end{prooftree}
		\quad
		\begin{prooftree}
		\hypo{$\Gamma$  $\vdash$  P(t/x)}
		\infer1{$\Gamma$  $\vdash$  $\exists$ xP(x)}
		\end{prooftree}
		\]
		
		\[
		\begin{prooftree}
		\hypo{P(c_{$\forall$ x.$\neg$ P(x)})$\vdash$ }
		\infer1{$\neg$ $\forall$ x.$\neg$ P(x) $\vdash$  }
		\end{prooftree}
		\quad
		\begin{prooftree}
		\hypo{$\vdash$ P(t)}
		\infer1{$\vdash$  $\neg$ $\forall$ x.$\neg$ P(x)}
		\end{prooftree}
		\quad
		\begin{prooftree}
		\hypo{P(t)$\vdash$ }
		\infer1{$\neg$ $\exists$ x.$\neg$ P(x) $\vdash$  }
		\end{prooftree}
		\quad
		\begin{prooftree}
		\hypo{$\vdash$ P(c_{$\exists$ x.$\neg$ P(x)})}
		\infer1{$\vdash$  $\neg$ $\exists$ x.$\neg$ P(x)}
		\end{prooftree}
		\]
	\end{center}

\section{Operational Rules}
	\begin{center}
				\subsection{Negation}
				\begin{center}
					\[
					\begin{prooftree}
					\hypo{ $\vdash$  A}
					\infer1{$\neg$  A $\vdash$ }
					\end{prooftree}
					\quad
					\begin{prooftree}
					\hypo{A $\vdash$  }
					\infer1{$\vdash$  $\neg$  A}
					\end{prooftree}
					\]
				\end{center}
				
				
				\subsection{Negative Junctions}
				\begin{center}
					\[
					\begin{prooftree}
					\hypo{$\vdash$  A}
					\hypo{$\vdash$  B}
					\infer2{$\neg$ A \vee $\neg$ B $\vdash$  }
					\end{prooftree}
					\quad
					\begin{prooftree}
					\hypo{A $\vdash$  }
					\infer1{ $\vdash$  $\neg$ A \vee $\neg$ B}
					\end{prooftree}
					\quad
					\begin{prooftree}
					\hypo{B $\vdash$  }
					\infer1{ $\vdash$  $\neg$ A \vee $\neg$ B}
					\end{prooftree}
					\]
					
					\[
					\begin{prooftree}
					\hypo{ $\vdash$  A}
					\infer1{$\neg$ A \wedge $\neg$ B $\vdash$  }
					\end{prooftree}
					\quad
					\begin{prooftree}
					\hypo{ $\vdash$  B}
					\infer1{$\neg$ A \wedge $\neg$ B $\vdash$  }
					\end{prooftree}
					\quad
					\begin{prooftree}
					\hypo{A $\vdash$  }
					\hypo{B $\vdash$  }
					\infer2{$\vdash$  $\neg$ A \wedge $\neg$ B}
					\end{prooftree}
					\]
				\end{center}

				\subsection{Conditionals}
				\begin{center}
					\[
					\begin{prooftree}
					\hypo{$\vdash$  A}
					\hypo{B $\vdash$  }
					\infer2{$\neg$ A \vee B $\vdash$ }
					\end{prooftree}
					\quad
					\begin{prooftree}
					\hypo{$\vdash$  A}
					\infer1{$\vdash$  $\neg$ A \vee B}
					\end{prooftree}
					\quad
					\begin{prooftree}
					\hypo{$\Gamma$  $\vdash$  B}
					\infer1{$\Gamma$ $\vdash$  A \vee B}
					\end{prooftree}
					\]
					
					\[
					\begin{prooftree}
					\hypo{A $\vdash$  $\Delta$ }
					\infer1{A \wedge $\neg$ B $\vdash$  $\Delta$ }
					\end{prooftree}
					\quad
					\begin{prooftree}
					\hypo{ $\vdash$  B}
					\infer1{A \wedge $\neg$ B $\vdash$  }
					\end{prooftree}
					\quad
					\begin{prooftree}
					\hypo{$\vdash$  A}
					\hypo{B $\vdash$  }
					\infer2{$\vdash$  A \wedge $\neg$ B}
					\end{prooftree}
					\]
				\end{center}
				
				\subsection{Junctions}
				\begin{center}
					\[
					\begin{prooftree}
					\hypo{A $\vdash$  $\Delta$ }
					\hypo{B $\vdash$  $\Delta$ }
					\infer2{A \vee B $\vdash$  $\Delta$ }
					\end{prooftree}
					\quad
					\begin{prooftree}
					\hypo{$\Gamma$  $\vdash$  A}
					\infer1{$\Gamma$  $\vdash$  A \vee B}
					\end{prooftree}
					\quad
					\begin{prooftree}
					\hypo{$\Gamma$  $\vdash$  B}
					\infer1{$\Gamma$  $\vdash$  A \vee B}
					\end{prooftree}
					\quad
					\begin{prooftree}
					\hypo{C $\vdash$  A, B}
					\infer1{C $\vdash$  A \vee B}
					\end{prooftree}
					\]
					
					\[
					\begin{prooftree}
					\hypo{A, B $\vdash$  C}
					\infer1{A \wedge B $\vdash$  C}
					\end{prooftree}
					\quad
					\begin{prooftree}
					\hypo{A $\vdash$  $\Delta$ }
					\infer1{A \wedge B $\vdash$  $\Delta$ }
					\end{prooftree}
					\quad
					\begin{prooftree}
					\hypo{B $\vdash$  $\Delta$ }
					\infer1{A \wedge B $\vdash$  $\Delta$ }
					\end{prooftree}
					\quad
					\begin{prooftree}
					\hypo{$\Gamma$  $\vdash$  A}
					\hypo{$\Gamma$  $\vdash$  B}
					\infer2{$\Gamma$  $\vdash$  A \wedge B}
					\end{prooftree}
					\]
				\end{center}
			
				\subsection{Biconditionals}
				\begin{center}
					\[
					\begin{prooftree}
					\hypo{$\vdash$  A}
					\hypo{B $\vdash$  }
					\infer2{($\neg$ A \vee B) \wedge ($\neg$ B \vee A) $\vdash$  }
					\end{prooftree}
					\quad
					\begin{prooftree}
					\hypo{A $\vdash$  }
					\hypo{B $\vdash$  }
					\infer2{ $\vdash$  ($\neg$ A \vee B) \wedge ($\neg$ B \vee A)}
					\end{prooftree}
					\quad
					\begin{prooftree}
					\hypo{$\Gamma$  $\vdash$  B}
					\hypo{$\Gamma$  $\vdash$  A}
					\infer2{$\Gamma$  $\vdash$  ($\neg$ A \vee B) \wedge ($\neg$ B \vee A)}
					\end{prooftree}
					\]
					
					\[
					\begin{prooftree}
					\hypo{A $\vdash$  }
					\hypo{$\vdash$ A}
					\infer2{(A \wedge B) \vee  ($\neg$ A \wedge $\neg$ B) $\vdash$  }
					\end{prooftree}
					\quad
					\begin{prooftree}
					\hypo{A $\vdash$  }
					\hypo{$\vdash$ B}
					\infer2{(A \wedge B) \vee  ($\neg$ A \wedge $\neg$ B) $\vdash$  }
					\end{prooftree}
					\quad
					\begin{prooftree}
					\hypo{B $\vdash$  }
					\hypo{$\vdash$ A}
					\infer2{(A \wedge B) \vee  ($\neg$ A \wedge $\neg$ B) $\vdash$  }
					\end{prooftree}
					\quad
					\begin{prooftree}
					\hypo{B $\vdash$  }
					\hypo{$\vdash$ B}
					\infer2{(A \wedge B) \vee  ($\neg$ A \wedge $\neg$ B) $\vdash$  }
					\end{prooftree}
					\]
					
					\[
					\quad
					\begin{prooftree}
					\hypo{$\Gamma$  $\vdash$  A}
					\hypo{$\Gamma$  $\vdash$  B}
					\infer2{$\Gamma$  $\vdash$  (A \wedge B) \vee  ($\neg$ A \wedge $\neg$ B)}
					\end{prooftree}
					\quad
					\begin{prooftree}
					\hypo{B $\vdash$  }
					\hypo{A $\vdash$  }
					\infer2{ $\vdash$  (A \wedge B) \vee  ($\neg$ A \wedge $\neg$ B)}
					\end{prooftree}
					\]
					
					TODO: XOR-like
					\[
					\begin{prooftree}
					\hypo{B $\vdash$  $\Delta$ }
					\hypo{A $\vdash$  $\Delta$ }
					\infer2{($\neg$ A \wedge B) \vee ($\neg$ B \vee A) $\vdash$  $\Delta$ }
					\end{prooftree}
					\quad
					\begin{prooftree}
					\hypo{$\vdash$  A}
					\hypo{$\vdash$  B}
					\infer2{($\neg$ A \wedge B) \vee ($\neg$ B \vee A) $\vdash$  }
					\end{prooftree}
					\quad
					\begin{prooftree}
					\hypo{A $\vdash$  }
					\hypo{$\vdash$  B}
					\infer2{($\neg$ A \wedge B) \vee ($\neg$ B \vee A) $\vdash$  }
					\end{prooftree}
					\quad
					\begin{prooftree}
					\hypo{$\vdash$  A}
					\hypo{B $\vdash$ }
					\infer2{($\neg$ A \wedge B) \vee ($\neg$ B \vee A) $\vdash$  }
					\end{prooftree}
					\]
					
					\[
					\quad
					\begin{prooftree}
					\hypo{A $\vdash$  }
					\hypo{$\vdash$  B}
					\infer2{ $\vdash$  ($\neg$ A \wedge B) \vee ($\neg$ B \vee A)}
					\end{prooftree}
					\quad
					\begin{prooftree}
					\hypo{$\vdash$  A}
					\hypo{B $\vdash$ }
					\infer2{$\vdash$  ($\neg$ A \wedge B) \vee ($\neg$ B \vee A)}
					\end{prooftree}
					\]
					
					\[
					\begin{prooftree}
					\hypo{$\vdash$  A}
					\hypo{$\vdash$  B}
					\infer2{(A \vee B) \wedge  ($\neg$ A \vee $\neg$ B) $\vdash$  }
					\end{prooftree}
					\quad
					\begin{prooftree}
					\hypo{A $\vdash$  $\Delta$ }
					\hypo{B $\vdash$  $\Delta$ }
					\infer2{(A \vee B) \wedge  ($\neg$ A \vee $\neg$ B) $\vdash$  $\Delta$ }
					\end{prooftree}
					\]
					
					\[
					\begin{prooftree}
					\hypo{$\vdash$  A}
					\hypo{A $\vdash$ }
					\infer2{$\vdash$  (A \vee B) \wedge  ($\neg$ A \vee $\neg$ B)}
					\end{prooftree}
					\quad
					\begin{prooftree}
					\hypo{$\vdash$  B}
					\hypo{B $\vdash$ }
					\infer2{$\vdash$  (A \vee B) \wedge  ($\neg$ A \vee $\neg$ B)}
					\end{prooftree}
					\quad
					\begin{prooftree}
					\hypo{$\vdash$  A}
					\hypo{B $\vdash$ }
					\infer2{$\vdash$  (A \vee B) \wedge  ($\neg$ A \vee $\neg$ B)}
					\end{prooftree}
					\quad
					\begin{prooftree}
					\hypo{$\vdash$  B}
					\hypo{A $\vdash$ }
					\infer2{$\vdash$  (A \vee B) \wedge  ($\neg$ A \vee $\neg$ B)}
					\end{prooftree}
					\quad
					\]
				\end{center}
\end{center}

\part{Theorems}
	\begin{center}
		
	\end{center}

