


\begin{abstract}

\end{abstract}

\section{Structural Rules}
Uses a variation of cut left.

\begin{center}
	\[
	\begin{prooftree}
	\infer0[Id]{A $\vdash$  A}
	\end{prooftree}
	\]
	
	\[
	\begin{prooftree}
	\hypo{$\Gamma$  $\vdash$  A}
	\hypo{$\Gamma$ _{L}, A, $\Gamma$ _{R} $\vdash$  C}
	\infer2[CutL]{$\Gamma$ _{L}, $\Gamma$ , $\Gamma$ _{R} $\vdash$  C}
	\end{prooftree}
	\]
\end{center}

\section{Operational Rules}
$$\Gamma$ $ non-empty in the RHS implication and negation rules.
\begin{center}
	
	\[
	\begin{prooftree}
	\hypo{$\Gamma$ _{L}, A, B, $\Gamma$ _{R} $\vdash$  C}
	\infer1{$\Gamma$ _{L}, A $\otimes$  B, $\Gamma$ _{R} $\vdash$  C}
	\end{prooftree}
	\quad
	\begin{prooftree}
	\hypo{$\Gamma$ _{L} $\vdash$  A}
	\hypo{$\Gamma$ _{R} $\vdash$  B}
	\infer2{$\Gamma$ _{L}, $\Gamma$ _{R} $\vdash$  A $\otimes$  B}
	\end{prooftree}
	\]
	
	\[
	\begin{prooftree}
	\hypo{$\Gamma$  $\vdash$  A}
	\hypo{$\Gamma$ _{L}, B, $\Gamma$ _{R} $\vdash$  C}
	\infer2{$\Gamma$ _{L}, $\Gamma$ , A $\to$  B, $\Gamma$ _{R} $\vdash$  C}
	\end{prooftree}
	\quad
	\begin{prooftree}
	\hypo{A, $\Gamma$  $\vdash$  B}
	\infer1{$\Gamma$  $\vdash$  A $\to$  B}
	\end{prooftree}
	\]
	
	\[
	\begin{prooftree}
	\hypo{$\Gamma$  $\vdash$  A}
	\hypo{$\Gamma$ _{L}, B, $\Gamma$ _{R} $\vdash$  C}
	\infer2{$\Gamma$ _{L}, B ← A, $\Gamma$ , $\Gamma$ _{R} $\vdash$  C}
	\end{prooftree}
	\quad
	\begin{prooftree}
	\hypo{$\Gamma$ , A $\vdash$  B}
	\infer1{$\Gamma$  $\vdash$  B ← A}
	\end{prooftree}
	\]
	
	\[
	\begin{prooftree}
	\hypo{ $\Gamma$  $\vdash$  A}
	\infer1{ $\neg$ _{L} A, $\Gamma$  $\vdash$  }
	\end{prooftree}
	\quad
	\begin{prooftree}
	\hypo{ $\Gamma$  $\vdash$  A}
	\infer1{ $\Gamma$ , $\neg$ _{R} A $\vdash$  }
	\end{prooftree}
	\quad
	\begin{prooftree}
	\hypo{ A, $\Gamma$  $\vdash$ _{L} }
	\infer1{ $\Gamma$  $\vdash$ _{L} $\neg$  A}
	\end{prooftree}
	\quad
	\begin{prooftree}
	\hypo{ $\Gamma$ , A $\vdash$ _{R} }
	\infer1{ $\Gamma$  $\vdash$ _{R} $\neg$  A}
	\end{prooftree}
	\]
\end{center}

\section{Theorems}
\begin{center}
	
	\[
	\begin{prooftree}
	\infer0{A $\vdash$  A}
	\infer1{A , $\neg$  A $\vdash$ }
	\infer1{A $\otimes$  $\neg$  A $\vdash$ }
	\end{prooftree}
	\quad
	\begin{prooftree}
	\infer0{A $\vdash$  A}
	\infer1{$\neg$  A, A $\vdash$ }
	\infer1{$\neg$  A $\otimes$  A$\vdash$ }
	\end{prooftree}
	\]
\end{center}

