





\usepackage[utf8]{inputenc}











































A sequent calculus of ordinary multiplicatives.


\section{Structural Rules}

\begin{center}
	\[
	\begin{prooftree}
	\infer0[Id]{A $\vdash$  A}
	\end{prooftree}
	\]
	
	\[
	\begin{prooftree}
	\hypo{$\Gamma$ _{L}, A $\vdash$ }
	\hypo{$\vdash$  $\Delta$ _{L}, A}
	\infer2[Cut]{$\Gamma$ _{L} $\vdash$  $\Delta$ _{L}}
	\end{prooftree}
	\]
	
	\[
	\begin{prooftree}
	\hypo{A, $\Gamma$ _{R} $\vdash$ }
	\hypo{$\vdash$  A, $\Delta$ _{R}}
	\infer2[Cut]{$\Gamma$ _{R} $\vdash$  $\Delta$ _{R}}
	\end{prooftree}
	\]
	\[
	\begin{prooftree}
	\hypo{$\Gamma$  $\vdash$  A}
	\hypo{A $\vdash$  $\Delta$ }
	\infer2[Cut]{$\Gamma$  $\vdash$  $\Delta$ }
	\end{prooftree}
	\]
	
	\[
	\begin{prooftree}
	\hypo{$\Gamma$ _{L}, A, $\Gamma$ _{R} $\vdash$ }
	\hypo{$\vdash$  $\Delta$ _{L}, A, $\Delta$ _{R}}
	\infer2[Cut]{$\Gamma$ _{L}, $\Gamma$ _{R} $\vdash$  $\Delta$ _{L}, $\Delta$ _{R}}
	\end{prooftree}
	\]
	
	\[
	\begin{prooftree}
	\hypo{$\Gamma$ _{L}, A, $\Gamma$ _{R} $\vdash$  $\Delta$ _{M}}
	\hypo{$\Gamma$ _{M} $\vdash$  $\Delta$ _{L}, A, $\Delta$ _{R}}
	\infer2[Cut]{$\Gamma$ _{L}, $\Gamma$ _{M}, $\Gamma$ _{R} $\vdash$  $\Delta$ _{L}, $\Delta$ _{M}, $\Delta$ _{R}}
	\end{prooftree}
	\]
\end{center}

\newpage
\section{Operational Rules}
\begin{center}
	\subsection{Negations}
	\begin{center}
		\[
		\begin{prooftree}
		\hypo{$\Gamma$ _{L}, $\Gamma$ _{R} $\vdash$  $\Delta$ _{L}, A, $\Delta$ _{R}}
		\infer1{$\Gamma$ _{L}, $\neg$ _{M} A, $\Gamma$ _{R} $\vdash$  $\Delta$ _{L}, $\Delta$ _{R}}
		\end{prooftree}
		\quad
		\begin{prooftree}
		\hypo{ $\Gamma$ _{L}, A, $\Gamma$ _{R} $\vdash$  $\Delta$ _{L}, $\Delta$ _{R}}
		\infer1{ $\Gamma$ _{L}, $\Gamma$ _{R} $\vdash$  $\Delta$ _{L}, $\neg$ _{M} A, $\Delta$ _{R}}
		\end{prooftree}
		\]
		
		\[
		\begin{prooftree}
		\hypo{$\Gamma$ _{L}, $\Gamma$ _{R} $\vdash$  A, $\Delta$ }
		\infer1{$\Gamma$ _{L}, $\neg$ _{L} A, $\Gamma$ _{R} $\vdash$  $\Delta$ }
		\end{prooftree}
		\quad
		\begin{prooftree}
		\hypo{A, $\Gamma$  $\vdash$  $\Delta$ _{L}, $\Delta$ _{R}}
		\infer1{ $\Gamma$  $\vdash$  $\Delta$ _{L}, $\neg$ _{L} A, $\Delta$ _{R}}
		\end{prooftree}
		\]
		
		\[
		\begin{prooftree}
		\hypo{$\Gamma$ _{L}, $\Gamma$ _{R} $\vdash$  $\Delta$ , A}
		\infer1{$\Gamma$ _{L}, $\neg$ _{R} A, $\Gamma$ _{R} $\vdash$  $\Delta$ }
		\end{prooftree}
		\quad
		\begin{prooftree}
		\hypo{ $\Gamma$ , A $\vdash$  $\Delta$ _{L}, $\Delta$ _{R}}
		\infer1{ $\Gamma$  $\vdash$  $\Delta$ _{L}, $\neg$ _{R} A, $\Delta$ _{R}}
		\end{prooftree}
		\]
		
		\[
		\begin{prooftree}
		\hypo{$\Gamma$  $\vdash$  A, $\Delta$ }
		\infer1{$\neg$ _{L} A, $\Gamma$  $\vdash$  $\Delta$ }
		\end{prooftree}
		\quad
		\begin{prooftree}
		\hypo{ A, $\Gamma$  $\vdash$  $\Delta$ }
		\infer1{ $\Gamma$  $\vdash$  $\neg$ _{L} A, $\Delta$ }
		\end{prooftree}
		\quad
		\begin{prooftree}
		\hypo{$\Gamma$  $\vdash$  $\Delta$ , A}
		\infer1{$\Gamma$ , $\neg$ _{R} A $\vdash$  $\Delta$ }
		\end{prooftree}
		\quad
		\begin{prooftree}
		\hypo{ $\Gamma$ , A $\vdash$  $\Delta$ }
		\infer1{ $\Gamma$  $\vdash$  $\Delta$ , $\neg$ _{R} A}
		\end{prooftree}
		\]
		
		\[
		\begin{prooftree}
		\hypo{$\Gamma$  $\vdash$  $\Delta$ , A}
		\infer1{$\neg$ ^{*}_{L} A, $\Gamma$  $\vdash$  $\Delta$ }
		\end{prooftree}
		\quad
		\begin{prooftree}
		\hypo{$\Gamma$ , A $\vdash$  $\Delta$ }
		\infer1{ $\Gamma$  $\vdash$  $\neg$ ^{*}_{L} A, $\Delta$ }
		\end{prooftree}
		\quad
		\begin{prooftree}
		\hypo{$\Gamma$  $\vdash$  A, $\Delta$ }
		\infer1{$\Gamma$ , $\neg$ ^{*}_{R} A $\vdash$  $\Delta$ }
		\end{prooftree}
		\quad
		\begin{prooftree}
		\hypo{ A, $\Gamma$  $\vdash$  $\Delta$ }
		\infer1{ $\Gamma$  $\vdash$  $\Delta$ , $\neg$ ^{*}_{R} A}
		\end{prooftree}
		\]
	\end{center}

	\subsection{Junctions}
	\begin{center}
		\[
		\begin{prooftree}
		\hypo{$\Gamma$ _{L}, A, B, $\Gamma$ _{R} $\vdash$  $\Delta$ }
		\infer1{$\Gamma$ _{L}, A $\otimes$  B, $\Gamma$ _{R} $\vdash$  $\Delta$ }
		\end{prooftree}
		\quad
		\begin{prooftree}
		\hypo{$\Gamma$ _{L} $\vdash$  $\Delta$ _{L}, A}
		\hypo{$\Gamma$ _{R} $\vdash$  B, $\Delta$ _{R}}
		\infer2{$\Gamma$ _{L}, $\Gamma$ _{R} $\vdash$  $\Delta$ _{L}, A $\otimes$  B, $\Delta$ _{R}}
		\end{prooftree}
		\]
		
		\[
		\begin{prooftree}
		\hypo{$\Gamma$ _{L}, B, A, $\Gamma$ _{R} $\vdash$  $\Delta$ }
		\infer1{$\Gamma$ _{L}, B $\otimes$  A, $\Gamma$ _{R} $\vdash$  $\Delta$ }
		\end{prooftree}
		\quad
		\begin{prooftree}
		\hypo{$\Gamma$ _{L} $\vdash$  $\Delta$ _{L}, B}
		\hypo{$\Gamma$ _{R} $\vdash$  A, $\Delta$ _{R}}
		\infer2{$\Gamma$ _{L}, $\Gamma$ _{R} $\vdash$  $\Delta$ _{L}, B $\otimes$  A, $\Delta$ _{R}}
		\end{prooftree}
		\]
		
		\[
		\begin{prooftree}
		\hypo{$\Gamma$ _{L}, B $\vdash$  $\Delta$ _{L}}
		\hypo{A, $\Gamma$ _{R} $\vdash$  $\Delta$ _{R}}
		\infer2{$\Gamma$ _{L}, B $\parr$  A, $\Gamma$ _{R} $\vdash$  $\Delta$ _{L}, $\Delta$ _{R}}
		\end{prooftree}
		\quad
		\begin{prooftree}
		\hypo{$\Gamma$  $\vdash$  $\Delta$ _{L}, B, A, $\Delta$ _{R}}
		\infer1{$\Gamma$  $\vdash$  $\Delta$ _{L}, B $\parr$  A, $\Delta$ _{R}}
		\end{prooftree}
		\]
		
		\[
		\begin{prooftree}
		\hypo{$\Gamma$ _{L}, A $\vdash$  $\Delta$ _{L}}
		\hypo{B, $\Gamma$ _{R} $\vdash$  $\Delta$ _{R}}
		\infer2{$\Gamma$ _{L}, A $\parr$  B, $\Gamma$ _{R} $\vdash$  $\Delta$ _{L}, $\Delta$ _{R}}
		\end{prooftree}
		\quad
		\begin{prooftree}
		\hypo{$\Gamma$  $\vdash$  $\Delta$ _{L}, A, B, $\Delta$ _{R}}
		\infer1{$\Gamma$  $\vdash$  $\Delta$ _{L}, A $\parr$  B, $\Delta$ _{R}}
		\end{prooftree}
		\]
	\end{center}
	\subsection{Conditionals}
		\begin{center}
			There are at least 4 kinds of implications possibly 5 if middle negation can be used. 
		\end{center}
		\subsection{Biconditionals}
			\begin{center}
				\[
				\begin{prooftree}
				\hypo{$\Gamma$ _{L}, $\neg$ A $\parr$  B, $\neg$ B $\parr$  A, $\Gamma$ _{R} $\vdash$  $\Delta$ _{L},$\Delta$ _{M},$\Delta$ _{R}}
				\infer1{$\Gamma$ _{L}, ($\neg$ A $\parr$  B)$\otimes$ ($\neg$ B $\parr$  A), $\Gamma$ _{R} $\vdash$  $\Delta$ _{L},$\Delta$ _{M},$\Delta$ _{R}}
				\end{prooftree}
				\quad
				\begin{prooftree}
				\hypo{$\Gamma$ _{L}, $\neg$ A $\vdash$  $\Delta$ _{L}}
				\hypo{B, $\neg$ B $\vdash$  $\Delta$ _{M}}
				\hypo{A, $\Gamma$ _{R} $\vdash$  $\Delta$ _{R}}
				\infer3{$\Gamma$ _{L}, ($\neg$ A $\parr$  B)$\otimes$ ($\neg$ B $\parr$  A), $\Gamma$ _{R} $\vdash$  $\Delta$ _{L},$\Delta$ _{M},$\Delta$ _{R}}
				\end{prooftree}
				\]
				
				\[
				\begin{prooftree}
				\hypo{$\Gamma$ _{L} $\vdash$  $\Delta$ _{L}, $\neg$ A , B}
				\hypo{$\Gamma$ _{R} $\vdash$  $\neg$ B , A, $\Delta$ _{R}}
				\infer2{$\Gamma$ _{L}, $\Gamma$ _{R} $\vdash$  $\Delta$ _{L}, ($\neg$ A $\parr$  B)$\otimes$ ($\neg$ B $\parr$  A), $\Delta$ _{R}}
				\end{prooftree}
				\]
				
				\[
				\begin{prooftree}
				\hypo{A, $\Gamma$ _{L} $\vdash$  $\Delta$ _{L}, B}
				\hypo{B, $\Gamma$ _{R} $\vdash$  A, $\Delta$ _{R}}
				\infer2{$\Gamma$ _{L}, $\Gamma$ _{R} $\vdash$  $\Delta$ _{L}, ($\neg$ _{L}A $\parr$  B)$\otimes$ ($\neg$ _{L}B $\parr$  A), $\Delta$ _{R}}
				\end{prooftree}
				\]
				
				\[
				\begin{prooftree}
				\hypo{$\Gamma$ _{L}, A $\vdash$  $\Delta$ _{L}, B}
				\hypo{$\Gamma$ _{R}, B $\vdash$  A, $\Delta$ _{R}}
				\infer2{$\Gamma$ _{L}, $\Gamma$ _{R} $\vdash$  $\Delta$ _{L}, ($\neg$ _{R}A $\parr$  B)$\otimes$ ($\neg$ _{R}B $\parr$  A), $\Delta$ _{R}}
				\end{prooftree}
				\]
				
				\[
				\begin{prooftree}
				\hypo{$\Gamma$ _{L}, A , B $\vdash$  $\Delta$ _{L}}
				\hypo{$\neg$ A , $\neg$ B, $\Gamma$ _{R} $\vdash$  $\Delta$ _{R}}
				\infer2{$\Gamma$ _{L}, (A $\otimes$  B)$\parr$ ($\neg$ A $\otimes$  $\neg$ B), $\Gamma$ _{R} $\vdash$  $\Delta$ _{L},$\Delta$ _{R}}
				\end{prooftree}
				\]
			\end{center}
\end{center}

\part{Theorems}
	\begin{center}
		
	\end{center}

