





\usepackage[utf8]{inputenc}











































A sequent system that preserves the law of excluded middle and non-contradiction, but not generally ECQ and EQN?


\section{Structural Rules}

\begin{center}
	\[
	\begin{prooftree}
	\infer0[Id]{A $\vdash$  A}
	\end{prooftree}
	\]
	
	\[
	\begin{prooftree}
	\hypo{$\Gamma$  $\vdash$  A}
	\hypo{$\Delta$ , A, $\Pi$  $\vdash$  C}
	\infer2[CutL]{$\Delta$ , $\Gamma$ , $\Pi$  $\vdash$  C}
	\end{prooftree}
	\quad
	\begin{prooftree}
	\hypo{$\Gamma$ , A, $\Phi$  $\vdash$  C}
	\hypo{C $\vdash$  $\Delta$ , A, $\Psi$ }
	\infer2[Cut]{$\Gamma$ , $\Phi$  $\vdash$  $\Delta$ , $\Psi$ }
	\end{prooftree}
	\quad
	\begin{prooftree}
	\hypo{C $\vdash$  $\Pi$ , A, $\Delta$ }
	\hypo{A $\vdash$  $\Gamma$ }
	\infer2[CutR]{C $\vdash$  $\Pi$ , $\Gamma$ , $\Delta$ }
	\end{prooftree}
	\]
\end{center}

\section{Unit Rules}
\begin{center}
		\[
	\begin{prooftree}
	\hypo{$\Gamma$ _{L}, $\Gamma$ _{R} $\vdash$  C}
	\infer1{$\Gamma$ _{L}, 1, $\Gamma$ _{R} $\vdash$  C}
	\end{prooftree}
	\quad
	\begin{prooftree}
	\hypo{C $\vdash$  $\Delta$ _{L}, $\Delta$ _{R}}
	\infer1{C $\vdash$  $\Delta$ _{L}, $\bot$ , $\Delta$ _{R}}
	\end{prooftree}
	\]
	
	\[
	\begin{prooftree}
	\infer0{ $\bot$  $\vdash$  }
	\end{prooftree}
	\quad
	\begin{prooftree}
	\infer0{ $\vdash$  1}
	\end{prooftree}
	\]
	
	\[
	\begin{prooftree}
	\infer0{$\Gamma$ _{L}, 0, $\Gamma$ _{R} $\vdash$  C}
	\end{prooftree}
	\quad
	\begin{prooftree}
	\infer0{ 0 $\vdash$  $\Delta$ }
	\end{prooftree}
	\quad
	\begin{prooftree}
	\infer0{ $\Gamma$  $\vdash$  $\top$ }
	\end{prooftree}
	\quad
	\begin{prooftree}
	\infer0{C $\vdash$  $\Delta$ _{L}, $\top$ , $\Delta$ _{R}}
	\end{prooftree}
	\]
	
	\[
	\begin{prooftree}
	\infer0{$\Gamma$ _{L}, 0, $\Gamma$ _{R} $\vdash$  $\Delta$ }
	\end{prooftree}
	\quad
	\begin{prooftree}
	\infer0{$\Gamma$  $\vdash$  $\Delta$ _{L}, $\top$ , $\Delta$ _{R}}
	\end{prooftree}
	\]
\end{center}

\newpage
\section{Operational Rules}
\begin{center}
	\subsection{Negations}
	\begin{center}
			\[
		\begin{prooftree}
		\hypo{$\Gamma$ , $\Phi$  $\vdash$  $\Delta$ , A, $\Psi$ }
		\infer1{$\Gamma$ , $\neg$  A, $\Phi$  $\vdash$  $\Delta$ , $\Psi$ }
		\end{prooftree}
		\quad
		\begin{prooftree}
		\hypo{ $\Phi$ , A, $\Gamma$  $\vdash$  $\Psi$ , $\Delta$ }
		\infer1{ $\Phi$ , $\Gamma$  $\vdash$  $\Psi$ , $\neg$  A, $\Delta$ }
		\end{prooftree}
		\quad
		\begin{prooftree}
		\hypo{$\Gamma$ , $\Phi$  $\vdash$  $\Delta$ , A, $\Psi$ }
		\infer1{$\Gamma$ , $\neg$  A, $\Phi$  $\vdash$  $\Delta$ , $\Psi$ }
		\end{prooftree}
		\quad
		\begin{prooftree}
		\hypo{$\Phi$ , A, $\Gamma$  $\vdash$  $\Psi$ , $\Delta$ }
		\infer1{ $\Phi$ , $\Gamma$  $\vdash$  $\Psi$ , $\neg$  A, $\Delta$ }
		\end{prooftree}
		\]
		
		\[
		\begin{prooftree}
		\hypo{$\Gamma$  $\vdash$  $\Delta$ , A}
		\infer1{$\Gamma$ , $\neg$  A $\vdash$  $\Delta$ }
		\end{prooftree}
		\quad
		\begin{prooftree}
		\hypo{ A, $\Gamma$  $\vdash$  $\Delta$ }
		\infer1{ $\Gamma$  $\vdash$  $\neg$  A, $\Delta$ }
		\end{prooftree}
		\]
		
		\[
		\begin{prooftree}
		\hypo{ $\Gamma$  $\vdash$  A}
		\infer1{ $\neg$  A, $\Gamma$  $\vdash$  }
		\end{prooftree}
		\quad
		\begin{prooftree}
		\hypo{ $\Gamma$  $\vdash$  A}
		\infer1{ $\Gamma$ , $\neg$  A$\vdash$  }
		\end{prooftree}
		\quad
		\begin{prooftree}
		\hypo{ A, $\Gamma$  $\vdash$  }
		\infer1{ $\Gamma$  $\vdash$  $\neg$  A}
		\end{prooftree}
		\quad
		\begin{prooftree}
		\hypo{ $\Gamma$ , A $\vdash$  }
		\infer1{ $\Gamma$  $\vdash$  $\neg$  A}
		\end{prooftree}
		\]
		
		\[
		\begin{prooftree}
		\hypo{ $\vdash$  A, $\Delta$ }
		\infer1{ $\neg$  A $\vdash$  $\Delta$ }
		\end{prooftree}
		\quad
		\begin{prooftree}
		\hypo{ $\vdash$  $\Delta$ , A}
		\infer1{ $\neg$  A$\vdash$  $\Delta$ }
		\end{prooftree}
		\quad
		\begin{prooftree}
		\hypo{ A $\vdash$  $\Delta$ }
		\infer1{ $\vdash$  $\neg$  A, $\Delta$ }
		\end{prooftree}
		\quad
		\begin{prooftree}
		\hypo{ A $\vdash$  $\Delta$ }
		\infer1{ $\vdash$  $\Delta$ , $\neg$  A}
		\end{prooftree}
		\]
	\end{center}

	\subsection{Additives}
	\begin{center}
		\[
		\begin{prooftree}
		\hypo{$\Gamma$ , A, $\Phi$  $\vdash$  $\Delta$ }
		\hypo{$\Gamma$ , B, $\Phi$  $\vdash$  $\Delta$ }
		\infer2{$\Gamma$ , A $\oplus$  B, $\Phi$  $\vdash$  $\Delta$ }
		\end{prooftree}
		\quad
		\begin{prooftree}
		\hypo{$\Gamma$  $\vdash$  $\Delta$ , A, $\Psi$  }
		\infer1{$\Gamma$  $\vdash$  $\Delta$ , A $\oplus$  B, $\Psi$ }
		\end{prooftree}
		\quad
		\begin{prooftree}
		\hypo{$\Gamma$  $\vdash$  $\Delta$ , B, $\Psi$  }
		\infer1{$\Gamma$  $\vdash$  $\Delta$ , A $\oplus$  B, $\Psi$ }
		\end{prooftree}
		\]
		
		\[
		\begin{prooftree}
		\hypo{$\Gamma$ , A, $\Phi$  $\vdash$  $\Psi$ }
		\infer1{$\Gamma$ , A \& B, $\Phi$  $\vdash$  $\Psi$ }
		\end{prooftree}
		\quad
		\begin{prooftree}
		\hypo{$\Gamma$ , B, $\Phi$  $\vdash$  $\Psi$ }
		\infer1{$\Gamma$ , A \& B, $\Phi$  $\vdash$  $\Psi$ }
		\end{prooftree}
		\quad
		\begin{prooftree}
		\hypo{ $\Gamma$  $\vdash$  $\Delta$ , B, $\Psi$ }
		\hypo{ $\Gamma$  $\vdash$  $\Delta$ , A, $\Psi$ }
		\infer2{ $\Gamma$  $\vdash$  $\Delta$ , B \& A, $\Psi$ }
		\end{prooftree}
		\]
		
		\[
		\begin{prooftree}
		\hypo{$\Gamma$ , A, $\Phi$  $\vdash$  C}
		\hypo{$\Gamma$ , B, $\Phi$  $\vdash$  C}
		\infer2{$\Gamma$ , A $\oplus$  B, $\Phi$  $\vdash$  C}
		\end{prooftree}
		\quad
		\begin{prooftree}
		\hypo{$\Gamma$  $\vdash$  A}
		\infer1{$\Gamma$  $\vdash$  A $\oplus$  B}
		\end{prooftree}
		\quad
		\begin{prooftree}
		\hypo{$\Gamma$  $\vdash$  B}
		\infer1{$\Gamma$  $\vdash$  A $\oplus$  B}
		\end{prooftree}
		\quad
		\begin{prooftree}
		\hypo{A $\vdash$  $\Delta$ }
		\infer1{A \& B $\vdash$  $\Delta$ }
		\end{prooftree}
		\quad
		\begin{prooftree}
		\hypo{B $\vdash$  $\Delta$ }
		\infer1{A \& B $\vdash$  $\Delta$ }
		\end{prooftree}
		\quad
		\begin{prooftree}
		\hypo{ C $\vdash$  $\Psi$ , B, $\Delta$ }
		\hypo{ C $\vdash$  $\Psi$ , A, $\Delta$ }
		\infer2{ C $\vdash$  $\Psi$ , B \& A, $\Delta$ }
		\end{prooftree}
		\]
		
		\[
		\begin{prooftree}
		\hypo{$\Gamma$ , A, $\Phi$  $\vdash$  C}
		\infer1{$\Gamma$ , A \& B, $\Phi$  $\vdash$  C}
		\end{prooftree}
		\quad
		\begin{prooftree}
		\hypo{$\Gamma$ , B, $\Phi$  $\vdash$  C}
		\infer1{$\Gamma$ , A \& B, $\Phi$  $\vdash$  C}
		\end{prooftree}
		\quad
		\begin{prooftree}
		\hypo{$\Gamma$  $\vdash$  A}
		\hypo{$\Gamma$  $\vdash$  B}
		\infer2{$\Gamma$  $\vdash$  A \& B}
		\end{prooftree}
		\quad
		\begin{prooftree}
		\hypo{B $\vdash$  $\Delta$ }
		\hypo{A $\vdash$  $\Delta$ }
		\infer2{B $\oplus$  A $\vdash$  $\Delta$ }
		\end{prooftree}
		\quad
		\begin{prooftree}
		\hypo{C $\vdash$  $\Psi$ , A, $\Delta$ }
		\infer1{C $\vdash$  $\Psi$ , B $\oplus$  A, $\Delta$ }
		\end{prooftree}
		\quad
		\begin{prooftree}
		\hypo{C $\vdash$  $\Psi$ , B, $\Delta$ }
		\infer1{C $\vdash$  $\Psi$ , B $\oplus$  A, $\Delta$ }
		\end{prooftree}
		\]
		
		
		\[
		\begin{prooftree}
		\hypo{$\Gamma$ , $\Phi$  $\vdash$  C, A}
		\hypo{$\Gamma$ , $\Phi$  $\vdash$  C, B}
		\infer2{$\Gamma$ , $\neg$  A $\oplus$  $\neg$  B, $\Phi$  $\vdash$  C}
		\end{prooftree}
		\quad
		\begin{prooftree}
		\hypo{A, $\Gamma$  $\vdash$  }
		\infer1{$\Gamma$  $\vdash$  $\neg$  A $\oplus$  $\neg$  B}
		\end{prooftree}
		\quad
		\begin{prooftree}
		\hypo{B, $\Gamma$  $\vdash$  }
		\infer1{$\Gamma$  $\vdash$  $\neg$  A $\oplus$  $\neg$  B}
		\end{prooftree}
		\quad
		\begin{prooftree}
		\hypo{$\vdash$  $\Delta$ , A}
		\infer1{$\neg$  B \& $\neg$  A $\vdash$  $\Delta$ }
		\end{prooftree}
		\quad
		\begin{prooftree}
		\hypo{$\vdash$  $\Delta$ , B}
		\infer1{$\neg$  B \& $\neg$  A $\vdash$  $\Delta$ }
		\end{prooftree}
		\quad
		\begin{prooftree}
		\hypo{ B, C $\vdash$  $\Psi$ , $\Delta$ }
		\hypo{ A, C $\vdash$  $\Psi$ , $\Delta$ }
		\infer2{ C $\vdash$  $\Psi$ , $\neg$  B \& $\neg$  A, $\Delta$ }
		\end{prooftree}
		\]
		
		\[
		\begin{prooftree}
		\hypo{$\Gamma$ , $\Phi$  $\vdash$  C, A}
		\infer1{$\Gamma$ , $\neg$  A \& $\neg$  B, $\Phi$  $\vdash$  C}
		\end{prooftree}
		\quad
		\begin{prooftree}
		\hypo{$\Gamma$ , $\Phi$  $\vdash$  C, B}
		\infer1{$\Gamma$ , $\neg$  A \& $\neg$  B, $\Phi$  $\vdash$  C}
		\end{prooftree}
		\quad
		\begin{prooftree}
		\hypo{A, $\Gamma$  $\vdash$  }
		\hypo{B, $\Gamma$  $\vdash$  }
		\infer2{$\Gamma$  $\vdash$  $\neg$  A \& $\neg$  B}
		\end{prooftree}
		\quad
		\begin{prooftree}
		\hypo{$\vdash$  $\Delta$ , B}
		\hypo{$\vdash$  $\Delta$ , A}
		\infer2{$\neg$  B $\oplus$  $\neg$  A $\vdash$  $\Delta$ }
		\end{prooftree}
		\quad
		\begin{prooftree}
		\hypo{A, C $\vdash$  $\Psi$ , $\Delta$ }
		\infer1{C $\vdash$  $\Psi$ , $\neg$  B $\oplus$  $\neg$  A, $\Delta$ }
		\end{prooftree}
		\quad
		\begin{prooftree}
		\hypo{B, C $\vdash$  $\Psi$ , $\Delta$ }
		\infer1{C $\vdash$  $\Psi$ , $\neg$  B $\oplus$  $\neg$  A, $\Delta$ }
		\end{prooftree}
		\]
		
	\end{center}

	\subsection{Multiplicatives}
	\begin{center}
		\[
		\begin{prooftree}
		\hypo{$\Gamma$ , A, B, $\Phi$  $\vdash$  C}
		\infer1{$\Gamma$ , A $\otimes$  B, $\Phi$  $\vdash$  C}
		\end{prooftree}
		\quad
		\begin{prooftree}
		\hypo{$\Gamma$  $\vdash$  A}
		\hypo{$\Phi$  $\vdash$  B}
		\infer2{$\Gamma$ , $\Phi$  $\vdash$  A $\otimes$  B}
		\end{prooftree}
		\quad
		\begin{prooftree}
		\hypo{B $\vdash$  $\Psi$ }
		\hypo{A $\vdash$  $\Delta$ }
		\infer2{B $\parr$  A $\vdash$  $\Psi$ , $\Delta$ }
		\end{prooftree}
		\quad
		\begin{prooftree}
		\hypo{C $\vdash$  $\Psi$ , B, A, $\Delta$ }
		\infer1{C $\vdash$  $\Psi$ , B $\parr$  A, $\Delta$ }
		\end{prooftree}
		\]
		
		\[
		\begin{prooftree}
		\hypo{$\Gamma$ , B, A, $\Phi$  $\vdash$  C}
		\infer1{$\Gamma$ , B $\otimes$  A, $\Phi$  $\vdash$  C}
		\end{prooftree}
		\quad
		\begin{prooftree}
		\hypo{$\Phi$  $\vdash$  B}
		\hypo{$\Gamma$  $\vdash$  A}
		\infer2{$\Phi$ , $\Gamma$  $\vdash$  B $\otimes$  A}
		\end{prooftree}
		\quad
		\begin{prooftree}
		\hypo{A $\vdash$  $\Delta$ }
		\hypo{B $\vdash$  $\Psi$ }
		\infer2{A $\parr$  B $\vdash$  $\Delta$ , $\Psi$ }
		\end{prooftree}
		\quad
		\begin{prooftree}
		\hypo{C $\vdash$  $\Psi$ , A, B, $\Delta$ }
		\infer1{C $\vdash$  $\Psi$ , A $\parr$  B, $\Delta$ }
		\end{prooftree}
		\]
		
		\[
		\begin{prooftree}
		\hypo{$\Gamma$  $\vdash$  A}
		\hypo{$\Phi$ , B, Θ $\vdash$  C}
		\infer2{$\Phi$ , $\Gamma$ , A $\to$  B, Θ $\vdash$  C}
		\end{prooftree}
		\quad
		\begin{prooftree}
		\hypo{A, $\Gamma$  $\vdash$  B}
		\infer1{$\Gamma$  $\vdash$  A $\to$  B}
		\end{prooftree}
		\quad
		\begin{prooftree}
		\hypo{B $\vdash$  $\Delta$ , A}
		\infer1{A $\nleftarrow$  B $\vdash$  $\Delta$ }
		\end{prooftree}
		\quad
		\begin{prooftree}
		\hypo{A $\vdash$  $\Delta$ }
		\hypo{C $\vdash$  Λ, B, $\Psi$ }
		\infer2{C $\vdash$  Λ, A $\nleftarrow$  B, $\Psi$ , $\Delta$ }
		\end{prooftree}
		\]
		
		\[
		\begin{prooftree}
		\hypo{$\Gamma$  $\vdash$  A}
		\hypo{$\Phi$ , B, Θ $\vdash$  C}
		\infer2{$\Phi$ , $\Gamma$ , B ← A, Θ $\vdash$  C}
		\end{prooftree}
		\quad
		\begin{prooftree}
		\hypo{$\Gamma$ , A $\vdash$  B}
		\infer1{$\Gamma$  $\vdash$  B ← A}
		\end{prooftree}
		\quad
		\begin{prooftree}
		\hypo{B $\vdash$  A, $\Psi$ }
		\infer1{A $\nrightarrow$  B $\vdash$  $\Psi$ }
		\end{prooftree}
		\quad
		\begin{prooftree}
		\hypo{A $\vdash$  $\Delta$ }
		\hypo{C $\vdash$  Λ, B, $\Psi$ }
		\infer2{C $\vdash$  Λ, B $\nrightarrow$  A, $\Psi$ , $\Delta$ }
		\end{prooftree}
		\]
	\end{center}
\end{center}

\part{Theorems}
	\begin{center}
		\[
		\begin{prooftree}
		\infer0{A $\vdash$  A}
		\infer1{1, A $\vdash$  A}
		\infer1{1 $\vdash$  A, $\neg$  A}
		\infer1{1 $\vdash$  A $\parr$  $\neg$  A}
		\end{prooftree}
		\quad
		\begin{prooftree}
		\infer0{A $\vdash$  A}
		\infer1{A, 1 $\vdash$  A}
		\infer1{A $\otimes$  1 $\vdash$  A}
		\end{prooftree}
		\quad
		\begin{prooftree}
		\infer0{A, 0 $\vdash$  A}
		\infer1{A $\otimes$  0 $\vdash$  A}
		\end{prooftree}
		\quad
		\begin{prooftree}
		\infer0{0 $\vdash$  A $\parr$  $\neg$  A}
		\end{prooftree}
		\]
		
		\[
		\begin{prooftree}
		\infer0{A $\vdash$  A}
		\infer1{A $\vdash$  A, $\bot$ }
		\infer1{A, $\neg$  A $\vdash$  $\bot$ }
		\infer1{A $\otimes$  $\neg$  A $\vdash$  $\bot$ }
		\end{prooftree}
		\quad
		\begin{prooftree}
		\infer0{A $\vdash$  A}
		\infer1{A $\vdash$  A, $\bot$ }
		\infer1{A $\vdash$  A $\parr$  $\bot$ }
		\end{prooftree}
		\quad
		\begin{prooftree}
		\infer0{A $\vdash$  A, $\top$ }
		\infer1{A $\vdash$  A $\parr$  $\top$ }
		\end{prooftree}
		\quad
		\begin{prooftree}
		\infer0{A $\otimes$  $\neg$  A $\vdash$  $\top$ }
		\end{prooftree}
		\]
		
		\[
		\begin{prooftree}
		\infer0{$\bot$  $\vdash$  }
		\infer1{$\bot$  $\vdash$  $\bot$ }
		\infer1{$\bot$ , $\neg$  $\bot$  $\vdash$  }
		\infer1{$\bot$  $\otimes$  $\neg$  $\bot$  $\vdash$  }
		\end{prooftree}
		\quad
		\begin{prooftree}
		\infer0{A $\vdash$  A}
		\infer1{A $\vdash$  A, $\bot$ }
		\infer1{A, $\neg$  $\bot$  $\vdash$  A}
		\infer1{A $\otimes$  $\neg$  $\bot$  $\vdash$  A}
		\end{prooftree}
		\quad
		\begin{prooftree}
		\infer0{ $\vdash$  1}
		\infer1{1 $\vdash$  1}
		\infer1{1, $\neg$  1 $\vdash$  }
		\infer1{1 $\otimes$  $\neg$  1 $\vdash$  }
		\end{prooftree}
		\quad
		\begin{prooftree}
		\infer0{A $\vdash$  A}
		\infer1{A, 1 $\vdash$  A}
		\infer1{1, $\neg$  A $\vdash$  $\neg$  A}
		\infer1{1 $\otimes$  $\neg$  A $\vdash$  $\neg$  A}
		\end{prooftree}
		\quad
		\begin{prooftree}
		\infer0{0 $\vdash$  $\Delta$ , A}
		\infer1{0, $\neg$  A $\vdash$  $\Delta$ }
		\infer1{0 $\otimes$  $\neg$  A $\vdash$  $\Delta$ }
		\end{prooftree}
		\quad
		\begin{prooftree}
		\infer0{A $\vdash$  $\Delta$ , $\top$ }
		\infer1{A, $\neg$  $\top$  $\vdash$  $\Delta$ }
		\infer1{A $\otimes$  $\neg$  $\top$  $\vdash$  $\Delta$ }
		\end{prooftree}
		\]
		
		\[
		\begin{prooftree}
		\infer0{A $\vdash$  A}
		\infer1{$\neg$ A $\vdash$  $\neg$ A}
		\infer1{$\neg$ A $\vdash$  $\neg$ A,  $\bot$ }
		\infer1{$\neg$ A $\vdash$  $\neg$ A $\parr$  $\bot$ }
		\end{prooftree}
		\quad
		\begin{prooftree}
		\infer0{A $\vdash$  A}
		\infer1{1, A $\vdash$  A}
		\infer1{A $\vdash$  A, $\neg$ 1}
		\infer1{A $\vdash$  A $\parr$  $\neg$ 1}
		\end{prooftree}
		\quad
		\begin{prooftree}
		\infer0{0, $\Gamma$  $\vdash$  A}
		\infer1{$\Gamma$  $\vdash$  A, $\neg$ 0}
		\infer1{$\Gamma$  $\vdash$  A $\parr$  $\neg$ 0}
		\end{prooftree}
		\quad
		\begin{prooftree}
		\infer0{A, $\Gamma$  $\vdash$  $\top$ }
		\infer1{ $\Gamma$ $\vdash$  $\top$ , $\neg$ A}
		\infer1{$\Gamma$  $\vdash$  $\top$  $\parr$  $\neg$ A}
		\end{prooftree}
		\]
		
		\[
		\begin{prooftree}
		\infer0{$\bot$  $\vdash$  }
		\infer1{$\bot$  $\vdash$  $\bot$ }
		\infer1{$\bot$ , $\neg$  $\bot$  $\vdash$  }
		\infer1{$\vdash$  $\bot$  $\parr$  $\neg$  $\bot$ }
		\end{prooftree}
		\quad
		\begin{prooftree}
		\infer0{ $\vdash$  1}
		\infer1{1 $\vdash$  1}
		\infer1{1, $\neg$  1 $\vdash$  }
		\infer1{1 $\otimes$  $\neg$  1 $\vdash$  }
		\end{prooftree}
		\quad
		\begin{prooftree}
		\infer0{0 $\vdash$  $\Delta$ , A}
		\infer1{0, $\neg$  A $\vdash$  $\Delta$ }
		\infer1{0 $\otimes$  $\neg$  A $\vdash$  $\Delta$ }
		\end{prooftree}
		\quad
		\begin{prooftree}
		\infer0{A $\vdash$  $\Delta$ , $\top$ }
		\infer1{A, $\neg$  $\top$  $\vdash$  $\Delta$ }
		\infer1{A $\otimes$  $\neg$  $\top$  $\vdash$  $\Delta$ }
		\end{prooftree}
		\]
		
		\[
		\begin{prooftree}
		\infer0{A $\vdash$  A}
		\infer1{A $\vdash$  A $\oplus$  $\neg$ A}
		\end{prooftree}
		\quad
		\begin{prooftree}
		\infer0{A $\vdash$  A}
		\infer1{ $\neg$  A \& A $\vdash$  A}
		\end{prooftree}
		\]
		
		\[
		\begin{prooftree}
		\infer0{A $\vdash$  A}
		\infer1{$\neg$  A, A $\vdash$ }
		\infer1{ $\neg$  A $\otimes$  A $\vdash$ }
		\end{prooftree}
		\quad
		\begin{prooftree}
		\infer0{A $\vdash$  A}
		\infer1{$\neg$  A, A $\vdash$ }
		\infer1{A $\otimes$  $\neg$  A $\vdash$ }
		\infer1{$\vdash$ $\neg$  (A $\otimes$  $\neg$  A)}
		\end{prooftree}
		\]

		\[
		\begin{prooftree}
		\infer0{A $\vdash$  A}
		\infer1{$\vdash$  A, $\neg$  A}
		\infer1{$\vdash$  A $\parr$  $\neg$  A}
		\end{prooftree}
		\quad
		\begin{prooftree}
		\infer0{A $\vdash$  A}
		\infer1{$\vdash$  A, $\neg$  A}
		\infer1{$\vdash$  A $\parr$  $\neg$  A}
		\infer1{$\neg$  (A $\parr$  $\neg$  A) $\vdash$ }
		\end{prooftree}
		\]

		\[
		\begin{prooftree}
		\infer0{$\bot$  $\vdash$ }
		\infer1{A \& $\bot$  $\vdash$ }
		\end{prooftree}
		\quad
		\begin{prooftree}
		\infer0{0 $\vdash$ }
		\infer1{A \& 0 $\vdash$ }
		\end{prooftree}
		\quad
		\begin{prooftree}
		\infer0{A $\vdash$  A}
		\infer0{A $\vdash$  $\top$ }
		\infer2{A $\vdash$  A \& $\top$ }
		\end{prooftree}
		\]
		
		\[
		\begin{prooftree}
		\infer0{$\vdash$  1}
		\infer1{$\vdash$  A $\oplus$  1}
		\end{prooftree}
		\quad
		\begin{prooftree}
		\infer0{$\vdash$  $\top$ }
		\infer1{$\vdash$  A $\oplus$  $\top$ }
		\end{prooftree}
		\quad
		\begin{prooftree}
		\infer0{A $\vdash$  A}
		\infer0{0 $\vdash$  A}
		\infer2{A $\oplus$  0 $\vdash$  A}
		\end{prooftree}
		\]
	\end{center}

