





\usepackage[utf8]{inputenc}





















Strictly visible additive order calculus.


\section{Structural Rules}

\begin{center}
	\[
	\begin{prooftree}
	\infer0[Id]{A $\vdash$  A}
	\end{prooftree}
	\]
	
	\[
	\begin{prooftree}
	\hypo{$\Gamma$  $\vdash$  A}
	\hypo{A $\vdash$  $\Delta$ }
	\infer2[cut]{$\Gamma$  $\vdash$  $\Delta$ }
	\end{prooftree}
	\]
\end{center}

\section{Operational Rules}
	\begin{center}
				\subsection{Negation}
				\begin{center}
					\[
					\begin{prooftree}
					\hypo{ $\vdash$  A}
					\infer1{$\neg$  A $\vdash$ }
					\end{prooftree}
					\quad
					\begin{prooftree}
					\hypo{A $\vdash$  }
					\infer1{$\vdash$  $\neg$  A}
					\end{prooftree}
					\]
				\end{center}
				
				
				\subsection{Negative Junctions}
				\begin{center}
					\[
					\begin{prooftree}
					\hypo{$\vdash$  A}
					\hypo{$\vdash$  B}
					\infer2{$\neg$ A $\oplus$  $\neg$ B $\vdash$  }
					\end{prooftree}
					\quad
					\begin{prooftree}
					\hypo{A $\vdash$  }
					\infer1{ $\vdash$  $\neg$ A $\oplus$  $\neg$ B}
					\end{prooftree}
					\quad
					\begin{prooftree}
					\hypo{B $\vdash$  }
					\infer1{ $\vdash$  $\neg$ A $\oplus$  $\neg$ B}
					\end{prooftree}
					\]
					
					\[
					\begin{prooftree}
					\hypo{$\vdash$  B}
					\hypo{ $\vdash$  A}
					\infer2{$\neg$ B $\oplus$  $\neg$ A $\vdash$  }
					\end{prooftree}
					\quad
					\begin{prooftree}
					\hypo{A $\vdash$  }
					\infer1{ $\vdash$  $\neg$ B $\oplus$  $\neg$ A}
					\end{prooftree}
					\quad
					\begin{prooftree}
					\hypo{B $\vdash$  }
					\infer1{ $\vdash$  $\neg$ B $\oplus$  $\neg$ A}
					\end{prooftree}
					\]
					
					\[
					\begin{prooftree}
					\hypo{ $\vdash$  A}
					\infer1{$\neg$ A \& $\neg$ B $\vdash$  }
					\end{prooftree}
					\quad
					\begin{prooftree}
					\hypo{ $\vdash$  B}
					\infer1{$\neg$ A \& $\neg$ B $\vdash$  }
					\end{prooftree}
					\quad
					\begin{prooftree}
					\hypo{A $\vdash$  }
					\hypo{B $\vdash$  }
					\infer2{$\vdash$  $\neg$ A \& $\neg$ B}
					\end{prooftree}
					\]
					
					\[
					\begin{prooftree}
					\hypo{ $\vdash$  A}
					\infer1{$\neg$ B \& $\neg$ A $\vdash$  }
					\end{prooftree}
					\quad
					\begin{prooftree}
					\hypo{ $\vdash$  B}
					\infer1{$\neg$ B \& $\neg$ A $\vdash$  }
					\end{prooftree}
					\quad
					\begin{prooftree}
					\hypo{B $\vdash$  }
					\hypo{A $\vdash$  }
					\infer2{ $\vdash$  $\neg$  B \& $\neg$  A}
					\end{prooftree}
					\]
				\end{center}

				\subsection{Conditionals}
				\begin{center}
					\[
					\begin{prooftree}
					\hypo{$\vdash$  B}
					\hypo{A $\vdash$  }
					\infer2{$\neg$ B $\oplus$  A $\vdash$ }
					\end{prooftree}
					\quad
					\begin{prooftree}
					\hypo{A $\vdash$  }
					\hypo{$\vdash$  B}
					\infer2{A $\oplus$  $\neg$ B $\vdash$ }
					\end{prooftree}
					\quad
					\begin{prooftree}
					\hypo{$\Gamma$  $\vdash$  A}
					\infer1{$\Gamma$  $\vdash$  A $\oplus$  $\neg$ B}
					\end{prooftree}
					\quad
					\begin{prooftree}
					\hypo{B $\vdash$  }
					\infer1{$\vdash$  A $\oplus$  $\neg$ B}
					\end{prooftree}
					\]
					
					\[
					\begin{prooftree}
					\hypo{ $\vdash$  A}
					\hypo{B $\vdash$  }
					\infer2{$\neg$ A $\oplus$  B $\vdash$  }
					\end{prooftree}
					\quad
					\begin{prooftree}
					\hypo{B $\vdash$  }
					\hypo{ $\vdash$  A}
					\infer2{B $\oplus$  $\neg$ A $\vdash$  }
					\end{prooftree}
					\quad
					\begin{prooftree}
					\hypo{A $\vdash$  }
					\infer1{ $\vdash$  B $\oplus$  $\neg$ A}
					\end{prooftree}
					\quad
					\begin{prooftree}
					\hypo{$\Gamma$  $\vdash$  B}
					\infer1{$\Gamma$  $\vdash$  B $\oplus$  $\neg$ A}
					\end{prooftree}
					\]
					
					\[
					\begin{prooftree}
					\hypo{A $\vdash$  $\Delta$ }
					\infer1{A \& $\neg$ B $\vdash$  $\Delta$ }
					\end{prooftree}
					\quad
					\begin{prooftree}
					\hypo{ $\vdash$  B}
					\infer1{A \& $\neg$ B $\vdash$  }
					\end{prooftree}
					\quad
					\begin{prooftree}
					\hypo{$\vdash$  A}
					\hypo{B $\vdash$  }
					\infer2{$\vdash$  A \& $\neg$ B}
					\end{prooftree}
					\quad
					\begin{prooftree}
					\hypo{B $\vdash$  }
					\hypo{$\vdash$  A}
					\infer2{$\vdash$  $\neg$ B \& A}
					\end{prooftree}
					\]
					
					\[
					\begin{prooftree}
					\hypo{ $\vdash$  A}
					\infer1{B \& $\neg$ A $\vdash$  }
					\end{prooftree}
					\quad
					\begin{prooftree}
					\hypo{B $\vdash$  $\Delta$ }
					\infer1{B \& $\neg$ A $\vdash$  $\Delta$ }
					\end{prooftree}
					\quad
					\begin{prooftree}
					\hypo{ $\vdash$  B}
					\hypo{A $\vdash$  }
					\infer2{ $\vdash$  B \& $\neg$  A}
					\end{prooftree}
					\quad
					\begin{prooftree}
					\hypo{A $\vdash$  }
					\hypo{ $\vdash$  B}
					\infer2{ $\vdash$  $\neg$ A \& B}
					\end{prooftree}
					\]
				\end{center}
				
				\subsection{Junctions}
				\begin{center}
					\[
					\begin{prooftree}
					\hypo{A $\vdash$  $\Delta$ }
					\hypo{B $\vdash$  $\Delta$ }
					\infer2{A $\oplus$  B $\vdash$  $\Delta$ }
					\end{prooftree}
					\quad
					\begin{prooftree}
					\hypo{$\Gamma$  $\vdash$  A}
					\infer1{$\Gamma$  $\vdash$  A $\oplus$  B}
					\end{prooftree}
					\quad
					\begin{prooftree}
					\hypo{$\Gamma$  $\vdash$  B}
					\infer1{$\Gamma$  $\vdash$  A $\oplus$  B}
					\end{prooftree}
					\]
					
					\[
					\begin{prooftree}
					\hypo{B $\vdash$  $\Delta$ }
					\hypo{A $\vdash$  $\Delta$ }
					\infer2{B $\oplus$  A $\vdash$  $\Delta$ }
					\end{prooftree}
					\quad
					\begin{prooftree}
					\hypo{$\Gamma$  $\vdash$  A}
					\infer1{$\Gamma$  $\vdash$  B $\oplus$  A}
					\end{prooftree}
					\quad
					\begin{prooftree}
					\hypo{$\Gamma$  $\vdash$  B}
					\infer1{$\Gamma$  $\vdash$  B $\oplus$  A}
					\end{prooftree}
					\]
					
					\[
					\begin{prooftree}
					\hypo{A $\vdash$  $\Delta$ }
					\infer1{A \& B $\vdash$  $\Delta$ }
					\end{prooftree}
					\quad
					\begin{prooftree}
					\hypo{B $\vdash$  $\Delta$ }
					\infer1{A \& B $\vdash$  $\Delta$ }
					\end{prooftree}
					\quad
					\begin{prooftree}
					\hypo{$\Gamma$  $\vdash$  A}
					\hypo{$\Gamma$  $\vdash$  B}
					\infer2{$\Gamma$  $\vdash$  A \& B}
					\end{prooftree}
					\]
					
					\[
					\begin{prooftree}
					\hypo{A $\vdash$  $\Delta$ }
					\infer1{B \& A $\vdash$  $\Delta$ }
					\end{prooftree}
					\quad
					\begin{prooftree}
					\hypo{B $\vdash$  $\Delta$ }
					\infer1{B \& A $\vdash$  $\Delta$ }
					\end{prooftree}
					\quad
					\begin{prooftree}
					\hypo{$\Gamma$  $\vdash$  B}
					\hypo{$\Gamma$  $\vdash$  A}
					\infer2{$\Gamma$  $\vdash$  B \& A}
					\end{prooftree}
					\]
				\end{center}
			
				\subsection{Biconditionals}
				\begin{center}
					\[
					\begin{prooftree}
					\hypo{$\vdash$  A}
					\hypo{B $\vdash$  }
					\infer2{($\neg$ A $\oplus$  B) \& ($\neg$ B $\oplus$  A) $\vdash$  }
					\end{prooftree}
					\quad
					\begin{prooftree}
					\hypo{$\vdash$  B}
					\hypo{A $\vdash$  }
					\infer2{($\neg$ A $\oplus$  B) \& ($\neg$ B $\oplus$  A) $\vdash$  }
					\end{prooftree}
					\quad
					\begin{prooftree}
					\hypo{A $\vdash$  }
					\hypo{B $\vdash$  }
					\infer2{ $\vdash$  ($\neg$ A $\oplus$  B) \& ($\neg$ B $\oplus$  A)}
					\end{prooftree}
					\quad
					\begin{prooftree}
					\hypo{$\Gamma$  $\vdash$  B}
					\hypo{$\Gamma$  $\vdash$  A}
					\infer2{$\Gamma$  $\vdash$  ($\neg$ A $\oplus$  B) \& ($\neg$ B $\oplus$  A)}
					\end{prooftree}
					\]
					
					\[
					\begin{prooftree}
					\hypo{A $\vdash$  }
					\hypo{$\vdash$ A}
					\infer2{(A \& B) $\oplus$   ($\neg$ A \& $\neg$ B) $\vdash$  }
					\end{prooftree}
					\quad
					\begin{prooftree}
					\hypo{A $\vdash$  }
					\hypo{$\vdash$ B}
					\infer2{(A \& B) $\oplus$   ($\neg$ A \& $\neg$ B) $\vdash$  }
					\end{prooftree}
					\quad
					\begin{prooftree}
					\hypo{B $\vdash$  }
					\hypo{$\vdash$ A}
					\infer2{(A \& B) $\oplus$   ($\neg$ A \& $\neg$ B) $\vdash$  }
					\end{prooftree}
					\quad
					\begin{prooftree}
					\hypo{B $\vdash$  }
					\hypo{$\vdash$ B}
					\infer2{(A \& B) $\oplus$   ($\neg$ A \& $\neg$ B) $\vdash$  }
					\end{prooftree}
					\]
					
					\[
					\quad
					\begin{prooftree}
					\hypo{$\Gamma$  $\vdash$  A}
					\hypo{$\Gamma$  $\vdash$  B}
					\infer2{$\Gamma$  $\vdash$  (A \& B) $\oplus$   ($\neg$ A \& $\neg$ B)}
					\end{prooftree}
					\quad
					\begin{prooftree}
					\hypo{B $\vdash$  }
					\hypo{A $\vdash$  }
					\infer2{ $\vdash$  (A \& B) $\oplus$   ($\neg$ A \& $\neg$ B)}
					\end{prooftree}
					\]
					
					TODO: XOR-like
				\end{center}
\end{center}

\part{Theorems}
	\begin{center}
	\end{center}

