





\usepackage[utf8]{inputenc}































Negation has partial visibility; the junctions obey strict visibility but the conditionals obey partial visibility.

	\begin{center}
		\section{Structural Rules}
			\begin{center}
				\[
				\begin{prooftree}
				\infer0[Id]{A $\vdash$  A}
				\end{prooftree}
				\]
				
				\[
				\begin{prooftree}
				\hypo{$\Gamma$  $\vdash$  A}
				\hypo{A $\vdash$  $\Delta$ }
				\infer2[cut]{$\Gamma$  $\vdash$  $\Delta$ }
				\end{prooftree}
				\]
			\end{center}
		
		\section{Operational Rules}
			\begin{center}
				Negations
				\[
				\begin{prooftree}
				\hypo{ $\vdash$  $\Delta$ , A}
				\infer1{$\neg$ _{R} A $\vdash$  $\Delta$ }
				\end{prooftree}
				\quad
				\begin{prooftree}
				\hypo{$\Gamma$ , A $\vdash$  }
				\infer1{$\Gamma$  $\vdash$  $\neg$ _{R} A}
				\end{prooftree}
				\]
				\[
				\begin{prooftree}
				\hypo{A, $\Gamma$  $\vdash$  }
				\infer1{$\Gamma$  $\vdash$  $\neg$ _{L} A}
				\end{prooftree}
				\quad
				\begin{prooftree}
				\hypo{ $\vdash$  A, $\Delta$ }
				\infer1{$\neg$ _{L} A $\vdash$  $\Delta$ }
				\end{prooftree}
				\]
				
				NANDs and NORs
				
				\[
				\begin{prooftree}
				\hypo{$\vdash$  A, $\Delta$ }
				\hypo{$\vdash$  B, $\Delta$ }
				\infer2{$\neg$ A $\oplus$  $\neg$ B $\vdash$  $\Delta$ }
				\end{prooftree}
				\quad
				\begin{prooftree}
				\hypo{$\Gamma$ , A $\vdash$  }
				\infer1{$\Gamma$  $\vdash$  $\neg$ A $\oplus$  $\neg$ B}
				\end{prooftree}
				\quad
				\begin{prooftree}
				\hypo{$\Gamma$ , B $\vdash$  }
				\infer1{$\Gamma$  $\vdash$  $\neg$ A $\oplus$  $\neg$ B}
				\end{prooftree}
				\]
				
				\[
				\begin{prooftree}
				\hypo{$\vdash$  B, $\Delta$ }
				\hypo{ $\vdash$  A, $\Delta$ }
				\infer2{$\neg$ B $\oplus$  $\neg$ A $\vdash$  $\Delta$ }
				\end{prooftree}
				\quad
				\begin{prooftree}
				\hypo{$\Gamma$ , A $\vdash$  }
				\infer1{$\Gamma$  $\vdash$  $\neg$ B $\oplus$  $\neg$ A}
				\end{prooftree}
				\quad
				\begin{prooftree}
				\hypo{$\Gamma$ , B $\vdash$  }
				\infer1{$\Gamma$  $\vdash$  $\neg$ B $\oplus$  $\neg$ A}
				\end{prooftree}
				\]
				
				\[
				\begin{prooftree}
				\hypo{ $\vdash$  A, $\Delta$ }
				\infer1{$\neg$ A \& $\neg$ B $\vdash$  $\Delta$ }
				\end{prooftree}
				\quad
				\begin{prooftree}
				\hypo{ $\vdash$  B, $\Delta$ }
				\infer1{$\neg$ A \& $\neg$ B $\vdash$  $\Delta$ }
				\end{prooftree}
				\quad
				\begin{prooftree}
				\hypo{$\Gamma$ ,A $\vdash$  }
				\hypo{$\Gamma$ ,B $\vdash$  }
				\infer2{$\Gamma$ $\vdash$  $\neg$ A \& $\neg$ B}
				\end{prooftree}
				\]
				
				\[
				\begin{prooftree}
				\hypo{ $\vdash$  A,$\Delta$ }
				\infer1{$\neg$ B \& $\neg$ A $\vdash$  $\Delta$ }
				\end{prooftree}
				\quad
				\begin{prooftree}
				\hypo{ $\vdash$  B,$\Delta$ }
				\infer1{$\neg$ B \& $\neg$ A $\vdash$  $\Delta$ }
				\end{prooftree}
				\quad
				\begin{prooftree}
				\hypo{$\Gamma$ , B $\vdash$  }
				\hypo{$\Gamma$ , A $\vdash$  }
				\infer2{$\Gamma$  $\vdash$  $\neg$  B \& $\neg$  A}
				\end{prooftree}
				\]
				
				Conditionals
				
				\[
				\begin{prooftree}
				\hypo{$\vdash$  B,$\Delta$ }
				\hypo{A $\vdash$  $\Delta$ }
				\infer2{$\neg$ B $\oplus$  A $\vdash$  $\Delta$ }
				\end{prooftree}
				\quad
				\begin{prooftree}
				\hypo{A $\vdash$  $\Delta$ }
				\hypo{$\vdash$  B,$\Delta$ }
				\infer2{A $\oplus$  $\neg$ B $\vdash$ $\Delta$ }
				\end{prooftree}
				\quad
				\begin{prooftree}
				\hypo{$\Gamma$  $\vdash$  A, $\Delta$ }
				\infer1{$\Gamma$  $\vdash$  A $\oplus$  $\neg$ B, $\Delta$ }
				\end{prooftree}
				\quad
				\begin{prooftree}
				\hypo{$\Gamma$ , B $\vdash$  }
				\infer1{$\Gamma$  $\vdash$  A $\oplus$  $\neg$ B}
				\end{prooftree}
				\]
				
				\[
				\begin{prooftree}
				\hypo{ $\vdash$  A, $\Delta$ }
				\hypo{B $\vdash$  $\Delta$ }
				\infer2{$\neg$ A $\oplus$  B $\vdash$  $\Delta$ }
				\end{prooftree}
				\quad
				\begin{prooftree}
				\hypo{B $\vdash$  $\Delta$ }
				\hypo{ $\vdash$  A, $\Delta$ }
				\infer2{B $\oplus$  $\neg$ A $\vdash$  $\Delta$ }
				\end{prooftree}
				\quad
				\begin{prooftree}
				\hypo{$\Gamma$ , A $\vdash$  }
				\infer1{$\Gamma$  $\vdash$  B $\oplus$  $\neg$ A}
				\end{prooftree}
				\quad
				\begin{prooftree}
				\hypo{$\Gamma$  $\vdash$  B, $\Delta$ }
				\infer1{$\Gamma$  $\vdash$  B $\oplus$  $\neg$ A, $\Delta$ }
				\end{prooftree}
				\]
				
				\[
				\begin{prooftree}
				\hypo{$\Gamma$ , A $\vdash$  $\Delta$ }
				\infer1{$\Gamma$ , A \& $\neg$ B $\vdash$  $\Delta$ }
				\end{prooftree}
				\quad
				\begin{prooftree}
				\hypo{ $\vdash$  B, $\Delta$ }
				\infer1{A \& $\neg$ B $\vdash$  $\Delta$ }
				\end{prooftree}
				\quad
				\begin{prooftree}
				\hypo{$\Gamma$ $\vdash$  A}
				\hypo{$\Gamma$ ,B $\vdash$  }
				\infer2{$\Gamma$ $\vdash$  A \& $\neg$ B}
				\end{prooftree}
				\quad
				\begin{prooftree}
				\hypo{$\Gamma$ ,B $\vdash$  }
				\hypo{$\Gamma$ $\vdash$  A}
				\infer2{$\Gamma$ $\vdash$  $\neg$ B \& A}
				\end{prooftree}
				\]
				
				\[
				\begin{prooftree}
				\hypo{ $\vdash$  A, $\Delta$ }
				\infer1{B \& $\neg$ A $\vdash$  $\Delta$ }
				\end{prooftree}
				\quad
				\begin{prooftree}
				\hypo{$\Gamma$ , B $\vdash$  $\Delta$ }
				\infer1{$\Gamma$ , B \& $\neg$ A $\vdash$  $\Delta$ }
				\end{prooftree}
				\quad
				\begin{prooftree}
				\hypo{$\Gamma$  $\vdash$  B}
				\hypo{$\Gamma$ ,A $\vdash$  }
				\infer2{$\Gamma$  $\vdash$  B \& $\neg$  A}
				\end{prooftree}
				\quad
				\begin{prooftree}
				\hypo{$\Gamma$ ,A $\vdash$  }
				\hypo{$\Gamma$  $\vdash$  B}
				\infer2{$\Gamma$  $\vdash$  $\neg$ A \& B}
				\end{prooftree}
				\]
				
				Conjunction and Disjunction
				
				\[
				\begin{prooftree}
				\hypo{A $\vdash$  $\Delta$ }
				\hypo{B $\vdash$  $\Delta$ }
				\infer2{A $\oplus$  B $\vdash$  $\Delta$ }
				\end{prooftree}
				\quad
				\begin{prooftree}
				\hypo{$\Gamma$  $\vdash$  A}
				\infer1{$\Gamma$  $\vdash$  A $\oplus$  B}
				\end{prooftree}
				\quad
				\begin{prooftree}
				\hypo{$\Gamma$  $\vdash$  B}
				\infer1{$\Gamma$  $\vdash$  A $\oplus$  B}
				\end{prooftree}
				\]
				
				\[
				\begin{prooftree}
				\hypo{B $\vdash$  $\Delta$ }
				\hypo{A $\vdash$  $\Delta$ }
				\infer2{B $\oplus$  A $\vdash$  $\Delta$ }
				\end{prooftree}
				\quad
				\begin{prooftree}
				\hypo{$\Gamma$  $\vdash$  A}
				\infer1{$\Gamma$  $\vdash$  B $\oplus$  A}
				\end{prooftree}
				\quad
				\begin{prooftree}
				\hypo{$\Gamma$  $\vdash$  B}
				\infer1{$\Gamma$  $\vdash$  B $\oplus$  A}
				\end{prooftree}
				\]
				
				\[
				\begin{prooftree}
				\hypo{A $\vdash$  $\Delta$ }
				\infer1{A \& B $\vdash$  $\Delta$ }
				\end{prooftree}
				\quad
				\begin{prooftree}
				\hypo{B $\vdash$  $\Delta$ }
				\infer1{A \& B $\vdash$  $\Delta$ }
				\end{prooftree}
				\quad
				\begin{prooftree}
				\hypo{$\Gamma$  $\vdash$  A}
				\hypo{$\Gamma$  $\vdash$  B}
				\infer2{$\Gamma$  $\vdash$  A \& B}
				\end{prooftree}
				\]
				
				\[
				\begin{prooftree}
				\hypo{A $\vdash$  $\Delta$ }
				\infer1{B \& A $\vdash$  $\Delta$ }
				\end{prooftree}
				\quad
				\begin{prooftree}
				\hypo{B $\vdash$  $\Delta$ }
				\infer1{B \& A $\vdash$  $\Delta$ }
				\end{prooftree}
				\quad
				\begin{prooftree}
				\hypo{$\Gamma$  $\vdash$  B}
				\hypo{$\Gamma$  $\vdash$  A}
				\infer2{$\Gamma$  $\vdash$  B \& A}
				\end{prooftree}
				\]
				Biconditionals
				\[
				\begin{prooftree}
				\hypo{$\vdash$  A, $\Delta$ }
				\hypo{B $\vdash$  $\Delta$ }
				\infer2{($\neg$ A $\oplus$  B) \& ($\neg$ B $\oplus$  A) $\vdash$  $\Delta$ }
				\end{prooftree}
				\quad
				\begin{prooftree}
				\hypo{$\vdash$  B, $\Delta$ }
				\hypo{A $\vdash$  $\Delta$ }
				\infer2{($\neg$ A $\oplus$  B) \& ($\neg$ B $\oplus$  A) $\vdash$  $\Delta$ }
				\end{prooftree}
				\quad
				\begin{prooftree}
				\hypo{$\Gamma$ , A $\vdash$  }
				\hypo{$\Gamma$ , B $\vdash$  }
				\infer2{$\Gamma$  $\vdash$  ($\neg$ A $\oplus$  B) \& ($\neg$ B $\oplus$  A)}
				\end{prooftree}
				\quad
				\begin{prooftree}
				\hypo{$\Gamma$  $\vdash$  B, $\Delta$ }
				\hypo{$\Gamma$  $\vdash$  A, $\Delta$ }
				\infer2{$\Gamma$  $\vdash$  ($\neg$ A $\oplus$  B) \& ($\neg$ B $\oplus$  A), $\Delta$ }
				\end{prooftree}
				\]
				
				\[
				\begin{prooftree}
				\hypo{A $\vdash$  $\Delta$ }
				\hypo{$\vdash$ A, $\Delta$ }
				\infer2{(A \& B) $\oplus$   ($\neg$ A \& $\neg$ B) $\vdash$  $\Delta$ }
				\end{prooftree}
				\quad
				\begin{prooftree}
				\hypo{A $\vdash$  $\Delta$ }
				\hypo{$\vdash$ B, $\Delta$ }
				\infer2{(A \& B) $\oplus$   ($\neg$ A \& $\neg$ B) $\vdash$  $\Delta$ }
				\end{prooftree}
				\quad
				\begin{prooftree}
				\hypo{B $\vdash$  $\Delta$ }
				\hypo{$\vdash$ A, $\Delta$ }
				\infer2{(A \& B) $\oplus$   ($\neg$ A \& $\neg$ B) $\vdash$  $\Delta$ }
				\end{prooftree}
				\quad
				\begin{prooftree}
				\hypo{B $\vdash$  $\Delta$ }
				\hypo{$\vdash$ B, $\Delta$ }
				\infer2{(A \& B) $\oplus$   ($\neg$ A \& $\neg$ B) $\vdash$  $\Delta$ }
				\end{prooftree}
				\]
				
				\[
				\quad
				\begin{prooftree}
				\hypo{$\Gamma$  $\vdash$  A, $\Delta$ }
				\hypo{$\Gamma$  $\vdash$  B, $\Delta$ }
				\infer2{$\Gamma$  $\vdash$  (A \& B) $\oplus$   ($\neg$ A \& $\neg$ B),$\Delta$ }
				\end{prooftree}
				\quad
				\begin{prooftree}
				\hypo{$\Gamma$ , B $\vdash$  }
				\hypo{$\Gamma$ , A $\vdash$  }
				\infer2{$\Gamma$  $\vdash$  (A \& B) $\oplus$   ($\neg$ A \& $\neg$ B)}
				\end{prooftree}
				\]
				
				TODO: Apartness
				
			\end{center}
		
		\part{Theorems}
			\begin{center}
			\end{center}
	\end{center}


