


\begin{abstract}

\end{abstract}

\section{Structural Rules}

\begin{center}
	\[
	\begin{prooftree}
	\infer0[Id]{A $\vdash$  A}
	\end{prooftree}
	\]
	
	\[
	\begin{prooftree}
	\hypo{$\Gamma$  $\vdash$  A}
	\hypo{A $\vdash$  $\Delta$ }
	\infer2[cut]{$\Gamma$  $\vdash$  $\Delta$ }
	\end{prooftree}
	\]
\end{center}

\section{Unit Rules}
\begin{center}
	\[
	\begin{prooftree}
	\infer0{0 $\vdash$  A}
	\end{prooftree}
	\quad
	\begin{prooftree}
	\infer0{A $\vdash$  $\top$ }
	\end{prooftree}
	\]
\end{center}

\section{Operational Rules}
\begin{center}
	\subsection{Additives}
	\begin{center}
		\[
		\begin{prooftree}
		\hypo{A $\vdash$  $\Delta$ }
		\hypo{B $\vdash$  $\Delta$ }
		\infer2{A $\oplus$  B $\vdash$  $\Delta$ }
		\end{prooftree}
		\quad
		\begin{prooftree}
		\hypo{$\Gamma$  $\vdash$  A}
		\infer1{$\Gamma$  $\vdash$  A $\oplus$  B}
		\end{prooftree}
		\quad
		\begin{prooftree}
		\hypo{$\Gamma$  $\vdash$  B}
		\infer1{$\Gamma$  $\vdash$  A $\oplus$  B}
		\end{prooftree}
		\]
		
		\[
		\begin{prooftree}
		\hypo{B $\vdash$  $\Delta$ }
		\hypo{A $\vdash$  $\Delta$ }
		\infer2{B $\oplus$  A $\vdash$  $\Delta$ }
		\end{prooftree}
		\quad
		\begin{prooftree}
		\hypo{$\Gamma$  $\vdash$  A}
		\infer1{$\Gamma$  $\vdash$  B $\oplus$  A}
		\end{prooftree}
		\quad
		\begin{prooftree}
		\hypo{$\Gamma$  $\vdash$  B}
		\infer1{$\Gamma$  $\vdash$  B $\oplus$  A}
		\end{prooftree}
		\]
	\end{center}
\end{center}

\part{Theorems}
	\begin{center}

		\[
		\begin{prooftree}
		\infer0{ $\vdash$  A $\oplus$  $\neg$ A}
		\end{prooftree}
		\quad
		\begin{prooftree}
		\infer0{ $\vdash$  $\neg$ A $\oplus$  A}
		\end{prooftree}
		\quad
		\begin{prooftree}
		\infer0{A \& $\neg$ A $\vdash$  }
		\end{prooftree}
		\quad
		\begin{prooftree}
		\infer0{$\neg$ A \& A $\vdash$  }
		\end{prooftree}
		\]
		
		\[
		\begin{prooftree}
		\infer0{0 $\vdash$  C}
		\infer1{0 \& $\neg$  A $\vdash$  C}
		\end{prooftree}
		\quad
		\begin{prooftree}
		\infer0{C $\vdash$  $\top$ }
		\infer1{C $\vdash$  $\top$  $\oplus$  $\neg$  A}
		\end{prooftree}		
		\]
		
		\[
		\begin{prooftree}
		\infer0{0 $\vdash$  A}
		\infer1{0 $\vdash$  A $\oplus$  $\neg$  A}
		\end{prooftree}
		\quad
		\begin{prooftree}
		\infer0{0 $\vdash$  $\neg$  A}
		\infer1{0 $\vdash$  A $\oplus$  $\neg$  A}
		\end{prooftree}
		\quad
		\begin{prooftree}
		\infer0{0 $\vdash$  }
		\infer1{$\vdash$  A $\oplus$  $\neg$  0}
		\end{prooftree}
		\quad
		\begin{prooftree}
		\infer0{C $\vdash$  $\top$ }
		\infer1{C $\vdash$  $\top$  $\oplus$  A}
		\end{prooftree}
		\]
		
		\[
		\begin{prooftree}
		\infer0{A $\vdash$  $\top$ }
		\infer1{A \& $\neg$  A $\vdash$  $\top$ }
		\end{prooftree}
		\quad
		\begin{prooftree}
		\infer0{$\neg$  A $\vdash$  $\top$ }
		\infer1{A \& $\neg$  A $\vdash$  $\top$ }
		\end{prooftree}
		\]
		
		\[
		\begin{prooftree}
		\infer0{1 $\vdash$  1}
		\infer1{1 $\vdash$  1 $\oplus$  $\neg$  1}
		\end{prooftree}
		\quad
		\begin{prooftree}
		\infer0{0 $\vdash$  1 $\oplus$  $\neg$  1}
		\end{prooftree}
		\quad
		\begin{prooftree}
		\hypo{$\bot$  $\vdash$  1 $\oplus$  $\neg$  1}
		\end{prooftree}
		\quad
		\begin{prooftree}
		\hypo{$\top$  $\vdash$  1 $\oplus$  $\neg$  1}
		\end{prooftree}
		\]
		
		\[
		\begin{prooftree}
		\infer0{$\bot$ $\vdash$ }
		\infer1{$\vdash$  $\neg$  $\bot$ }
		\infer1{$\vdash$  $\bot$  $\oplus$  $\neg$  $\bot$ }
		\infer1{1 $\vdash$  $\bot$  $\oplus$  $\neg$  $\bot$ }
		\end{prooftree}
		\quad
		\begin{prooftree}
		\infer0{0 $\vdash$  $\bot$  $\oplus$  $\neg$  $\bot$ }
		\end{prooftree}
		\quad
		\begin{prooftree}
		\infer0{$\bot$  $\vdash$  $\bot$ }
		\infer1{$\bot$  $\vdash$  $\bot$  $\oplus$  $\neg$  $\bot$ }
		\end{prooftree}
		\quad
		\begin{prooftree}
		\hypo{$\top$  $\vdash$  $\bot$  $\oplus$  $\neg$  $\bot$ }
		\end{prooftree}
		\]
		
		\[
		\begin{prooftree}
		\infer0{0 $\vdash$ }
		\infer1{$\vdash$  $\neg$  0}
		\infer1{$\vdash$  0 $\oplus$  $\neg$  0}
		\infer1{1 $\vdash$  0 $\oplus$  $\neg$  0}
		\end{prooftree}
		\quad
		\begin{prooftree}
		\infer0{0 $\vdash$  0 $\oplus$  $\neg$  0}
		\end{prooftree}
		\quad
		\begin{prooftree}
		\hypo{$\bot$  $\vdash$  0 $\oplus$  $\neg$  0}
		\end{prooftree}
		\quad
		\begin{prooftree}
		\hypo{$\top$  $\vdash$  0 $\oplus$  $\neg$  0}
		\end{prooftree}
		\]
		
		\[
		\begin{prooftree}
		\infer0{$\vdash$  $\top$ }
		\infer1{$\vdash$  $\top$  $\oplus$  $\neg$  $\top$ }
		\infer1{1 $\vdash$  $\top$  $\oplus$  $\neg$  $\top$ }
		\end{prooftree}
		\quad
		\begin{prooftree}
		\infer0{0 $\vdash$  $\top$  $\oplus$  $\neg$  $\top$ }
		\end{prooftree}
		\quad
		\begin{prooftree}
		\infer0{$\bot$  $\vdash$  $\top$ }
		\infer1{$\bot$  $\vdash$  $\top$  $\oplus$  $\neg$  $\top$ }
		\end{prooftree}
		\quad
		\begin{prooftree}
		\infer0{$\top$  $\vdash$  $\top$ }
		\infer1{$\top$  $\vdash$  $\top$  $\oplus$  $\neg$  $\top$ }
		\end{prooftree}
		\]
		
		\[
		\begin{prooftree}
		\infer0{1 $\vdash$  1}
		\infer1{1 \&  $\neg$  1$\vdash$  1}
		\end{prooftree}
		\quad
		\begin{prooftree}
		\hypo{1 \&  $\neg$  1$\vdash$  0}
		\end{prooftree}
		\quad
		\begin{prooftree}
		\infer0{$\vdash$  1}
		\infer1{$\neg$  1$\vdash$  }
		\infer1{1 \&  $\neg$  1$\vdash$  }
		\infer1{1 \&  $\neg$  1$\vdash$  $\bot$ }
		\end{prooftree}
		\quad
		\begin{prooftree}
		\infer0{1 \&  $\neg$  1 $\vdash$  $\top$ }
		\end{prooftree}
		\]
		
		\[
		\begin{prooftree}
		\infer0{0 $\vdash$  1}
		\infer1{0 \&  $\neg$  0 $\vdash$  1}
		\end{prooftree}
		\quad
		\begin{prooftree}
		\infer0{0 $\vdash$  0}
		\infer1{0 \&  $\neg$  0 $\vdash$  0}
		\end{prooftree}
		\quad
		\begin{prooftree}
		\infer0{0 $\vdash$  $\bot$ }
		\infer1{0 \&  $\neg$  0 $\vdash$  $\bot$ }
		\end{prooftree}
		\quad
		\begin{prooftree}
		\infer0{0 \&  $\neg$  0 $\vdash$  $\top$ }
		\end{prooftree}
		\]
		
		\[
		\begin{prooftree}
		\hypo{$\bot$  \&  $\neg$  $\bot$  $\vdash$  1}
		\end{prooftree}
		\quad
		\begin{prooftree}
		\hypo{$\bot$  \&  $\neg$  $\bot$  $\vdash$  0}
		\end{prooftree}
		\quad
		\begin{prooftree}
		\infer0{$\bot$  $\vdash$  }
		\infer1{$\bot$  \&  $\neg$  $\bot$  $\vdash$  }
		\infer1{$\bot$  \&  $\neg$  $\bot$  $\vdash$  $\bot$ }
		\end{prooftree}
		\quad
		\begin{prooftree}
		\infer0{$\bot$  \&  $\neg$  $\bot$  $\vdash$  $\top$ }
		\end{prooftree}
		\]
		
		\[
		\begin{prooftree}
		\hypo{$\top$  \&  $\neg$  $\top$  $\vdash$  1}
		\end{prooftree}
		\quad
		\begin{prooftree}
		\hypo{$\top$  \&  $\neg$  $\top$  $\vdash$  0}
		\end{prooftree}
		\quad
		\begin{prooftree}
		\infer0{$\vdash$  $\top$ }
		\infer1{$\neg$  $\top$  $\vdash$ }
		\infer1{$\neg$  $\top$  $\vdash$  $\bot$ }
		\infer1{$\top$  \&  $\neg$  $\top$  $\vdash$  $\bot$ }
		\end{prooftree}
		\quad
		\begin{prooftree}
		\infer0{$\top$  \&  $\neg$  $\top$  $\vdash$  $\top$ }
		\end{prooftree}
		\]
	\end{center}

